Add documentation

BFS/BFS.thy
@@ -1,9 +1,23 @@
 theory BFS
   imports
-    "../Graph_Theory/Directed_Graphs/Directed_Graphs"
-    "../Map_Specs_Tbd"
-    "../Tbd"
+    "../Graph/Adjacency/Directed_Adjacency"
+    "../Graph/Directed_Graph/Directed_Graph"
+    "../Map/Map_Specs_Ext"
+    "../Map/Parent_Relation"
+    "../Queue/Queue_Specs"
 begin
+
+text \<open>
+This theory specifies and verifies breadth-first search (BFS). More specifically, we verify that
+given a directed graph G and a source vertex src, the output of the algorithm induces a
+breadth-first tree T, that is, T consists of the vertices reachable from src in G, and for every
+vertex v in T, T contains a unique simple path from src to v that is also a shortest path from src
+to v in G.
+\<close>
+
+section \<open>BFS\<close>
+
+subsection \<open>Specification of the algorithm\<close>
 
 record ('q, 'm) state =
   queue :: 'q
@@ -40,7 +54,13 @@ locale bfs =
   Q_list
 begin
 
-section \<open>Algorithm\<close>
+text \<open>
+Our implementation of BFS keeps two data structures, a first-in, first-out queue, initialized to
+contain the source vertex src, and a parent map, initialized to the empty map. As long as the queue
+is not empty, the algorithm pops the head u of the queue, and for every adjacent vertex v, discovers
+v if it hasn't been discovered yet, where discovering v entails enqueuing v as well as setting v's
+parent to u.
+\<close>
 
 definition init :: "'a \<Rightarrow> ('q, 'm) state" where
   "init src \<equiv>
@@ -50,8 +70,8 @@ definition init :: "'a \<Rightarrow> ('q, 'm) state" where
 definition DONE :: "('q, 'm) state \<Rightarrow> bool" where
   "DONE s \<longleftrightarrow> Q_is_empty (queue s)"
 
-definition discovered :: "'a \<Rightarrow> 'm \<Rightarrow> 'a \<Rightarrow> bool" where
-  "discovered src m v \<longleftrightarrow> v = src \<or> P_lookup m v \<noteq> None"
+definition is_discovered :: "'a \<Rightarrow> 'm \<Rightarrow> 'a \<Rightarrow> bool" where
+  "is_discovered src m v \<longleftrightarrow> v = src \<or> P_lookup m v \<noteq> None"
 
 definition discover :: "'a \<Rightarrow> 'a \<Rightarrow> ('q, 'm) state \<Rightarrow> ('q, 'm) state" where
   "discover u v s \<equiv>
@@ -60,7 +80,7 @@ definition discover :: "'a \<Rightarrow> 'a \<Rightarrow> ('q, 'm) state \<Right
 
 definition traverse_edge :: "'a \<Rightarrow> 'a \<Rightarrow> 'a \<Rightarrow> ('q, 'm) state \<Rightarrow> ('q, 'm) state" where
   "traverse_edge src u v s \<equiv>
-   if \<not> discovered src (parent s) v then discover u v s
+   if \<not> is_discovered src (parent s) v then discover u v s
    else s"
 
 function (domintros) loop :: "'n \<Rightarrow> 'a \<Rightarrow> ('q, 'm) state \<Rightarrow> ('q, 'm) state" where
@@ -69,7 +89,7 @@ function (domintros) loop :: "'n \<Rightarrow> 'a \<Rightarrow> ('q, 'm) state \
     then let
           u = Q_head (queue s);
           q = Q_tail (queue s)
-         in loop G src (fold (traverse_edge src u) (G.adjacency G u) (s\<lparr>queue := q\<rparr>))
+         in loop G src (fold (traverse_edge src u) (G.adjacency_list G u) (s\<lparr>queue := q\<rparr>))
     else s)"
   by pat_completeness simp
 
@@ -80,602 +100,25 @@ abbreviation fold :: "'n \<Rightarrow> 'a \<Rightarrow> ('q, 'm) state \<Rightar
   "fold G src s \<equiv>
    List.fold
     (traverse_edge src (Q_head (queue s)))
-    (G.adjacency G (Q_head (queue s)))
+    (G.adjacency_list G (Q_head (queue s)))
     (s\<lparr>queue := Q_tail (queue s)\<rparr>)"
 
 abbreviation T :: "'m \<Rightarrow> 'a dgraph" where
   "T m \<equiv> {(u, v). P_lookup m v = Some u}"
 
-section \<open>Convenience Lemmas\<close>
-
-subsection \<open>@{term "Q_invar \<circ> queue"}\<close>
-
-lemma invar_tail:
-  assumes "Q_invar (queue s)"
-  assumes "\<not> DONE s"
-  shows "Q_invar (queue (s\<lparr>queue := Q_tail (queue s)\<rparr>))"
-  using assms Q.invar_tail
-  by (simp add: DONE_def Q.is_empty)
-
-subsection \<open>@{term "Q_list \<circ> queue"}\<close>
-
-lemma list_queue_non_empty:
-  assumes "Q_invar (queue s)"
-  assumes "\<not> DONE s"
-  shows "Q_list (queue s) \<noteq> []"
-  using assms
-  by (simp add: DONE_def Q.is_empty)
-
-subsection \<open>@{term "Q_head \<circ> queue"}\<close>
-
-lemma head_queue_mem_dV:
-  assumes "Q_invar (queue s)"
-  assumes "set (Q_list (queue s)) \<subseteq> G.dV G"
-  assumes "\<not> DONE s"
-  shows "Q_head (queue s) \<in> G.dV G"
-  using assms list_queue_non_empty
-  by (auto simp add: Q.list_head)
-
-section \<open>Basic Lemmas\<close>
-
-subsection \<open>@{term discover}\<close>
-
-subsubsection \<open>@{term queue}\<close>
-
-lemma queue_discover_cong [simp]:
-  shows "queue (discover u v s) = Q_snoc (queue s) v"
-  by (simp add: discover_def)
-
-subsubsection \<open>@{term parent}\<close>
-
-lemma parent_discover_cong [simp]:
-  shows "parent (discover u v s) = P_update v u (parent s)"
-  by (simp add: discover_def)
-
-subsection \<open>@{term traverse_edge}\<close>
-
-subsubsection \<open>@{term queue}\<close>
-
-lemma queue_traverse_edge_cong:
-  shows "queue (traverse_edge src u v s) = (if \<not> discovered src (parent s) v then Q_snoc (queue s) v else queue s)"
-  by (simp add: traverse_edge_def)
-
-subsubsection \<open>@{term "Q_invar \<circ> queue"}\<close>
-
-lemma invar_queue_traverse_edge:
-  assumes "Q_invar (queue s)"
-  shows "Q_invar (queue (traverse_edge src u v s))"
-  using assms Q.invar_snoc
-  by (simp add: queue_traverse_edge_cong)
-
-subsubsection \<open>@{term "Q_list \<circ> queue"}\<close>
-
-lemma list_queue_traverse_edge_cong:
-  assumes "Q_invar (queue s)"
-  shows
-    "Q_list (queue (traverse_edge src u v s)) =
-     Q_list (queue s) @ (if \<not> discovered src (parent s) v then [v] else [])"
-  using assms
-  by (simp add: queue_traverse_edge_cong Q.list_snoc)
-
-subsubsection \<open>@{term "P_lookup \<circ> parent"}\<close>
-
-lemma lookup_parent_traverse_edge_cong:
-  assumes "P_invar (parent s)"
-  shows
-    "P_lookup (parent (traverse_edge src u v s)) =
-     override_on
-      (P_lookup (parent s))
-      (\<lambda>_. Some u)
-      (if \<not> discovered src (parent s) v then {v} else {})"
-  using assms
-  by (simp add: traverse_edge_def P.map_update override_on_insert')
-
-subsubsection \<open>@{term "P_invar \<circ> parent"}\<close>
-
-lemma invar_parent_traverse_edge:
-  assumes "P_invar (parent s)"
-  shows "P_invar (parent (traverse_edge src u v s))"
-  using assms P.invar_update
-  by (simp add: traverse_edge_def)
-
-subsubsection \<open>@{term T}\<close>
-
-lemma T_traverse_edge_cong:
-  assumes "P_invar (parent s)"
-  shows "T (parent (traverse_edge src u v s)) = T (parent s) \<union> (if \<not> discovered src (parent s) v then {(u, v)} else {})"
-  using assms
-  by (auto simp add: lookup_parent_traverse_edge_cong override_on_def discovered_def)
-
-subsection \<open>@{term fold}\<close>
-
-subsubsection \<open>@{term "Q_invar \<circ> queue"}\<close>
-
-lemma invar_queue_fold:
-  assumes "Q_invar (queue s)"
-  assumes "distinct l"
-  shows "Q_invar (queue (List.fold (traverse_edge src u) l s))"
-  using assms
-  by (induct l arbitrary: s) (simp_all add: invar_queue_traverse_edge)
-
-lemma invar_queue_fold_2:
-  assumes "G.invar G"
-  assumes "Q_invar (queue s)"
-  assumes "\<not> DONE s"
-  shows "Q_invar (queue (fold G src s))"
-  using assms
-  by (auto intro: G.distinct_adjacency invar_tail invar_queue_fold)
-
-subsubsection \<open>@{term "Q_list \<circ> queue"}\<close>
-
-lemma list_queue_fold_cong_aux:
-  assumes "P_invar (parent s)"
-  assumes "distinct (v # vs)"
-  shows "filter (Not \<circ> discovered src (parent (traverse_edge src u v s))) vs = filter (Not \<circ> discovered src (parent s)) vs"
-proof (rule filter_cong)
-  fix w
-  assume "w \<in> set vs"
-  hence "discovered src (parent (traverse_edge src u v s)) w = discovered src (parent s) w"
-    using assms
-    by (auto simp add: discovered_def lookup_parent_traverse_edge_cong override_on_insert')
-  thus "(Not \<circ> discovered src (parent (traverse_edge src u v s))) w = (Not \<circ> discovered src (parent s)) w"
-    by simp
-qed simp
-
-lemma list_queue_fold_cong:
-  assumes "Q_invar (queue s)"
-  assumes "P_invar (parent s)"
-  assumes "distinct l"
-  shows
-    "Q_list (queue (List.fold (traverse_edge src u) l s)) =
-     Q_list (queue s) @ filter (Not \<circ> discovered src (parent s)) l"
-  using assms
-proof (induct l arbitrary: s)
-  case Nil
-  thus ?case
-    by simp
-next
-  case (Cons v vs)
-  have
-    "Q_list (queue (List.fold (traverse_edge src u) (v # vs) s)) =
-     Q_list (queue (List.fold (traverse_edge src u) vs (traverse_edge src u v s)))"
-    by simp
-  also have
-    "... =
-     Q_list (queue (traverse_edge src u v s)) @
-     filter (Not \<circ> discovered src (parent (traverse_edge src u v s))) vs"
-    using Cons.prems
-    by (auto intro: invar_queue_traverse_edge invar_parent_traverse_edge Cons.hyps)
-  also have
-    "... =
-     Q_list (queue s) @
-     (if \<not> discovered src (parent s) v then [v] else []) @
-     filter (Not \<circ> discovered src (parent (traverse_edge src u v s))) vs"
-    using Cons.prems(1)
-    by (simp add: list_queue_traverse_edge_cong)
-  also have
-    "... =
-     Q_list (queue s) @
-     (if \<not> discovered src (parent s) v then [v] else []) @
-     filter (Not \<circ> discovered src (parent s)) vs"
-    using Cons.prems(2, 3)
-    by (simp add: list_queue_fold_cong_aux)
-  also have "... = Q_list (queue s) @ filter (Not \<circ> discovered src (parent s)) (v # vs)"
-    by simp
-  finally show ?case
-    .
-qed
-
-lemma list_queue_fold_cong_2:
-  assumes "G.invar G"
-  assumes "Q_invar (queue s)"
-  assumes "P_invar (parent s)"
-  assumes "\<not> DONE s"
-  shows
-    "Q_list (queue (fold G src s)) =
-     Q_list (Q_tail (queue s)) @
-     filter (Not \<circ> discovered src (parent s)) (G.adjacency G (Q_head (queue s)))"
-proof -
-  have
-    "Q_list (queue (fold G src s)) =
-     Q_list (queue (s\<lparr>queue := Q_tail (queue s)\<rparr>)) @
-     filter
-      (Not \<circ> discovered src (parent (s\<lparr>queue := Q_tail (queue s)\<rparr>)))
-      (G.adjacency G (Q_head (queue s)))"
-    using assms
-    by (intro invar_tail G.distinct_adjacency list_queue_fold_cong) simp+
-  thus ?thesis
-    unfolding comp_apply
-    by (simp add: discovered_def)
-qed
-
-subsubsection \<open>@{term "set \<circ> Q_list \<circ> queue"}\<close>
-
-lemma queue_fold_subset_dV:
-  assumes "G.invar G"
-  assumes "Q_invar (queue s)"
-  assumes "P_invar (parent s)"
-  assumes "set (Q_list (queue s)) \<subseteq> G.dV G"
-  assumes "\<not> DONE s"
-  shows "set (Q_list (queue (fold G src s))) \<subseteq> G.dV G"
-proof
-  fix v
-  assume assm: "v \<in> set (Q_list (queue (fold G src s)))"
-  show "v \<in> G.dV G"
-  proof (cases "v \<in> set (filter (Not \<circ> discovered src (parent s)) (G.adjacency G (Q_head (queue s))))")
-    case True
-    thus ?thesis
-      using G.adjacency_subset_dV
-      by auto
-  next
-    case False
-    hence "v \<in> set (Q_list (Q_tail (queue s)))"
-      using assms assm
-      by (auto simp add: list_queue_fold_cong_2)
-    hence "v \<in> set (Q_list (queue s))"
-      using assms(2, 5) list_queue_non_empty
-      by (auto simp add: Q.list_tail intro: list.set_sel(2))
-    thus ?thesis
-      using assms(4)
-      by blast
-  qed
-qed
-
-subsubsection \<open>@{term parent}\<close>
-
-lemma lookup_parent_fold_cong:
-  assumes "P_invar (parent s)"
-  assumes "distinct l"
-  shows
-    "P_lookup (parent (List.fold (traverse_edge src u) l s)) =
-     override_on
-      (P_lookup (parent s))
-      (\<lambda>_. Some u)
-      (set (filter (Not \<circ> discovered src (parent s)) l))"
-  using assms
-proof (induct l arbitrary: s)
-  case Nil
-  thus ?case
-    by simp
-next
-  case (Cons v vs)
-  have
-    "P_lookup (parent (List.fold (traverse_edge src u) (v # vs) s)) =
-     P_lookup (parent (List.fold (traverse_edge src u) vs (traverse_edge src u v s)))"
-    by simp
-  also have
-    "... =
-     override_on
-      (P_lookup (parent (traverse_edge src u v s)))
-      (\<lambda>_. Some u)
-      (set (filter (Not \<circ> discovered src (parent (traverse_edge src u v s))) vs))"
-    using Cons.prems
-    by (fastforce intro: invar_parent_traverse_edge Cons.hyps)
-  also have
-    "... =
-     override_on
-      (override_on (P_lookup (parent s)) (\<lambda>_. Some u) (if \<not> discovered src (parent s) v then {v} else {}))
-      (\<lambda>_. Some u)
-      (set (filter (Not \<circ> discovered src (parent (traverse_edge src u v s))) vs))"
-    using Cons.prems(1)
-    by (simp add: lookup_parent_traverse_edge_cong)
-  also have
-    "... =
-     override_on
-      (override_on (P_lookup (parent s)) (\<lambda>_. Some u) (if \<not> discovered src (parent s) v then {v} else {}))
-      (\<lambda>_. Some u)
-      (set (filter (Not \<circ> discovered src (parent s)) vs))"
-    using Cons.prems
-    by (simp add: list_queue_fold_cong_aux)
-  finally show ?case
-    by (simp add: override_on_insert')
-qed
-
-lemma lookup_parent_fold_cong_2:
-  assumes "G.invar G"
-  assumes "P_invar (parent s)"
-  shows
-    "P_lookup (parent (fold G src s)) =
-     override_on
-      (P_lookup (parent s))
-      (\<lambda>_. Some (Q_head (queue s)))
-      (set (filter (Not \<circ> discovered src (parent s)) (G.adjacency G (Q_head (queue s)))))"
-proof -
-  have
-    "P_lookup (parent (fold G src s)) =
-     override_on
-      (P_lookup (parent (s\<lparr>queue := Q_tail (queue s)\<rparr>)))
-      (\<lambda>_. Some (Q_head (queue s)))
-      (set (filter (Not \<circ> discovered src (parent (s\<lparr>queue := Q_tail (queue s)\<rparr>))) (G.adjacency G (Q_head (queue s)))))"
-    using assms
-    by (intro G.distinct_adjacency lookup_parent_fold_cong) simp+
-  thus ?thesis
-    by (simp add: discovered_def)
-qed
-
-subsubsection \<open>@{term "P_invar \<circ> parent"}\<close>
-
-lemma invar_parent_fold:
-  assumes "P_invar (parent s)"
-  assumes "distinct l"
-  shows "P_invar (parent (List.fold (traverse_edge src u) l s))"
-  using assms
-  by (induct l arbitrary: s) (simp_all add: invar_parent_traverse_edge)
-
-lemma invar_parent_fold_2:
-  assumes "G.invar G"
-  assumes "P_invar (parent s)"
-  shows "P_invar (parent (fold G src s))"
-  using assms
-  by (intro G.distinct_adjacency invar_parent_fold) simp+
-
-subsubsection \<open>@{term "P.dom \<circ> parent"}\<close>
-
-lemma dom_parent_fold_subset_dV:
-  assumes "P_invar (parent s)"
-  assumes "distinct l"
-  assumes "P.dom (parent s) \<subseteq> G.dV G"
-  assumes "set l \<subseteq> G.dV G"
-  shows "P.dom (parent (List.fold (traverse_edge src u) l s)) \<subseteq> G.dV G"
-proof
-  fix v
-  assume assm: "v \<in> P.dom (parent (List.fold (traverse_edge src u) l s))"
-  show "v \<in> G.dV G"
-  proof (cases "v \<in> set (filter (Not \<circ> discovered src (parent s)) l)")
-    case True
-    thus ?thesis
-      using assms(4)
-      by auto
-  next
-    case False
-    have "P_lookup (parent (List.fold (traverse_edge src u) l s)) v \<noteq> None"
-      using assm
-      by (simp add: P.dom_def)
-    hence "P_lookup (parent s) v \<noteq> None"
-      using assms(1, 2) False
-      by (simp add: lookup_parent_fold_cong)
-    thus ?thesis
-      using assms(3)
-      by (auto simp add: P.dom_def)
-  qed
-qed
-
-lemma dom_parent_fold_subset_dV_2:
-  assumes "G.invar G"
-  assumes "P_invar (parent s)"
-  assumes "P.dom (parent s) \<subseteq> G.dV G"
-  shows "P.dom (parent (fold G src s)) \<subseteq> G.dV G"
-  using assms G.adjacency_subset_dV
-  by (intro G.distinct_adjacency dom_parent_fold_subset_dV) simp+
-
-subsubsection \<open>@{term "P.ran \<circ> parent"}\<close>
-
-lemma ran_parent_fold_cong:
-  assumes "G.invar G"
-  assumes "P_invar (parent s)"
-  shows
-    "P.ran (parent (fold G src s)) =
-     P.ran (parent s) \<union>
-     (if set (filter (Not \<circ> discovered src (parent s)) (G.adjacency G (Q_head (queue s)))) = {}
-      then {}
-      else {Q_head (queue s)})"
-proof
-  let ?S = "set (filter (Not \<circ> discovered src (parent s)) (G.adjacency G (Q_head (queue s))))"
-  show "P.ran (parent (fold G src s)) \<subseteq> P.ran (parent s) \<union> (if ?S = {} then {} else {Q_head (queue s)})"
-    using assms
-    by (auto simp add: P.ran_def lookup_parent_fold_cong_2 override_on_def)
-  show "P.ran (parent s) \<union> (if ?S = {} then {} else {Q_head (queue s)}) \<subseteq> P.ran (parent (fold G src s))"
-  proof
-    fix u
-    assume assm: "u \<in> P.ran (parent s) \<union> (if ?S = {} then {} else {Q_head (queue s)})"
-    show "u \<in> P.ran (parent (fold G src s))"
-    proof (cases "u \<in> P.ran (parent s)")
-      case True
-      then obtain v where
-        "P_lookup (parent s) v = Some u"
-        by (auto simp add: P.ran_def)
-      moreover hence "discovered src (parent s) v"
-        by (simp add: discovered_def)
-      ultimately show ?thesis
-        using assms
-        by (auto simp add: P.ran_def lookup_parent_fold_cong_2 override_on_def)
-    next
-      case False
-      then obtain v where
-        "v \<in> ?S"
-        using assm
-        by (auto split: if_splits(2))
-      moreover have "u = Q_head (queue s)"
-        using assm False
-        by (simp split: if_splits(2))
-      ultimately show ?thesis
-        using assms
-        by (auto simp add: P.ran_def lookup_parent_fold_cong_2 override_on_def)
-    qed
-  qed
-qed
-
-subsubsection \<open>@{term T}\<close>
-
-lemma T_fold_cong_aux:
-  assumes "P_invar (parent s)"
-  assumes "distinct (v # vs)"
-  shows "w \<in> set vs \<and> \<not> discovered src (parent (traverse_edge src u v s)) w \<longleftrightarrow> w \<in> set vs \<and> \<not> discovered src (parent s) w"
-  using assms
-  by (auto simp add: discovered_def lookup_parent_traverse_edge_cong override_on_def)
-
-lemma T_fold_cong:
-  assumes "P_invar (parent s)"
-  assumes "distinct l"
-  shows "T (parent (List.fold (traverse_edge src u) l s)) = T (parent s) \<union> {(u, v) |v. v \<in> set l \<and> \<not> discovered src (parent s) v}"
-  using assms
-proof (induct l arbitrary: s)
-  case Nil
-  thus ?case
-    by auto
-next
-  case (Cons v vs)
-  have
-    "T (parent (List.fold (traverse_edge src u) (v # vs) s)) =
-     T (parent (List.fold (traverse_edge src u) vs (traverse_edge src u v s)))"
-    by simp
-  also have
-    "... =
-     T (parent (traverse_edge src u v s)) \<union>
-     {(u, w) |w. w \<in> set vs \<and> \<not> discovered src (parent (traverse_edge src u v s)) w}"
-    using Cons.prems
-    by (intro invar_parent_traverse_edge Cons.hyps) simp+
-  also have
-    "... =
-     T (parent s) \<union>
-     (if \<not> discovered src (parent s) v then {(u, v)} else {}) \<union>
-     {(u, w) |w. w \<in> set vs \<and> \<not> discovered src (parent (traverse_edge src u v s)) w}"
-    unfolding T_traverse_edge_cong[OF Cons.prems(1)]
-    by blast
-  also have
-    "... =
-     T (parent s) \<union>
-     (if \<not> discovered src (parent s) v then {(u, v)} else {}) \<union>
-     {(u, w) |w. w \<in> set vs \<and> \<not> discovered src (parent s) w}"
-    using Cons.prems
-    by (simp add: T_fold_cong_aux)
-  also have "... = T (parent s) \<union> {(u, w) |w. w \<in> set (v # vs) \<and> \<not> discovered src (parent s) w}"
-    by force
-  finally show ?case
-    .
-qed
-
-lemma T_fold_cong_2:
-  assumes "G.invar G"
-  assumes "P_invar (parent s)"
-  shows
-    "T (parent (fold G src s)) =
-     T (parent s) \<union>
-     {(Q_head (queue s), v) |v. v \<in> set (G.adjacency G (Q_head (queue s))) \<and> \<not> discovered src (parent s) v}"
-proof -
-  have
-    "T (parent (fold G src s)) =
-     T (parent (s\<lparr>queue := Q_tail (queue s)\<rparr>)) \<union>
-     {(Q_head (queue s), v) |v.
-      v \<in> set (G.adjacency G (Q_head (queue s))) \<and>
-      \<not> discovered src (parent (s\<lparr>queue := Q_tail (queue s)\<rparr>)) v}"
-    using assms
-    by (intro G.distinct_adjacency T_fold_cong) simp+
-  thus ?thesis
-    by (simp add: discovered_def)
-qed
-
-section \<open>Termination\<close>
-
-lemma loop_dom_aux:
-  assumes "G.invar G"
-  assumes "P_invar (parent s)"
-  assumes "P.dom (parent s) \<subseteq> G.dV G"
-  shows
-    "card (P.dom (parent (fold G src s))) =
-     card (P.dom (parent s)) +
-     card (set (filter (Not \<circ> discovered src (parent s)) (G.adjacency G (Q_head (queue s)))))"
-proof -
-  let ?S = "set (filter (Not \<circ> discovered src (parent s)) (G.adjacency G (Q_head (queue s))))"
-  have "P.dom (parent (fold G src s)) = P.dom (parent s) \<union> ?S"
-    using assms(1, 2)
-    by (auto simp add: P.dom_def lookup_parent_fold_cong_2 override_on_def)
-  moreover have "finite (P.dom (parent s))"
-    using assms(1, 3) finite_subset
-    by (fastforce intro: G.finite_dV)
-  moreover have "finite ?S"
-    by simp
-  moreover have "P.dom (parent s) \<inter> ?S = {}"
-    by (auto simp add: P.dom_def discovered_def)
-  ultimately show ?thesis
-    by (simp add: card_Un_disjoint)
-qed
-
-lemma loop_dom_aux_2:
-  assumes invar_G: "G.invar G"
-  assumes invar_queue: "Q_invar (queue s)"
-  assumes not_DONE: "\<not> DONE s"
-  assumes dom_parent_subset_dV: "P.dom (parent s) \<subseteq> G.dV G"
-  shows
-    "card (G.dV G) +
-     length (Q_list (Q_tail (queue s))) -
-     card (P.dom (parent s)) <
-     card (G.dV G) +
-     length (Q_list (queue s)) -
-     card (P.dom (parent s))"
-proof -
-  have "Q_list (queue s) \<noteq> []"
-    using invar_queue not_DONE
-    by (intro list_queue_non_empty)
-  hence "length (Q_list (Q_tail (queue s))) < length (Q_list (queue s))"
-    using invar_queue
-    by (simp add: Q.list_tail)
-  moreover have "card (P.dom (parent s)) \<le> card (G.dV G)"
-    using invar_G dom_parent_subset_dV
-    by (intro G.finite_dV card_mono)
-  ultimately show ?thesis
-    by simp
-qed
-
-lemma loop_dom:
-  assumes "G.invar G"
-  assumes "Q_invar (queue s)"
-  assumes "P_invar (parent s)"
-  assumes "set (Q_list (queue s)) \<subseteq> G.dV G"
-  assumes "P.dom (parent s) \<subseteq> G.dV G"
-  shows "loop_dom (G, src, s)"
-  using assms
-proof (induct "card (G.dV G) + length (Q_list (queue s)) - card (P.dom (parent s))"
-       arbitrary: s
-       rule: less_induct)
-  case less
-  show ?case
-  proof (cases "DONE s")
-    case True
-    thus ?thesis
-      by (blast intro: loop.domintros)
-  next
-    case False
-    let ?u = "Q_head (queue s)"
-    let ?q = "Q_tail (queue s)"
-    let ?S = "set (filter (Not \<circ> discovered src (parent s)) (G.adjacency G (Q_head (queue s))))"
-
-    have "length (Q_list (queue (fold G src s))) = length (Q_list ?q) + card ?S"
-      using less.prems(1-3) False G.distinct_adjacency
-      by (simp add: list_queue_fold_cong_2 distinct_card[symmetric])
-    moreover have "card (P.dom (parent (fold G src s))) = card (P.dom (parent s)) + card ?S"
-      using less.prems(1, 3, 5)
-      by (intro loop_dom_aux)
-    ultimately have
-      "card (G.dV G) + length (Q_list (queue (fold G src s))) - card (P.dom (parent (fold G src s))) =
-       card (G.dV G) + length (Q_list ?q) + card ?S - (card (P.dom (parent s)) + card ?S)"
-      by presburger
-    also have "... = card (G.dV G) + length (Q_list ?q) - card (P.dom (parent s))"
-      by simp
-    also have "... < card (G.dV G) + length (Q_list (queue s)) - card (P.dom (parent s))"
-      using less.prems False
-      by (intro loop_dom_aux_2)
-    finally have
-      "card (G.dV G) + length (Q_list (queue (fold G src s))) - card (P.dom (parent (fold G src s))) <
-       card (G.dV G) + length (Q_list (queue s)) - card (P.dom (parent s))"
-      .
-    thus ?thesis
-      using less.prems
-      by (intro invar_queue_fold_2 invar_parent_fold_2 queue_fold_subset_dV dom_parent_fold_subset_dV_2 less.hyps loop.domintros)
-  qed
-qed
-
 end
 
-section \<open>Invariants\<close>
+subsection \<open>Verification of the correctness of the algorithm\<close>
 
-subsection \<open>Definitions\<close>
+subsubsection \<open>Input\<close>
 
-(* TODO Rename. *)
-abbreviation (in bfs) rev_follow :: "'m \<Rightarrow> 'a \<Rightarrow> 'a dpath" where
-  "rev_follow m v \<equiv> rev (parent.follow (P_lookup m) v)"
+text \<open>
+Algorithm @{term bfs.bfs} expects a directed graph G and a source vertex src in G as input, and the
+correctness theorem will assume such an input. We remark that the assumption that src is indeed a
+vertex in G is for the purpose of convenience. Let us formally specify these assumptions.
+\<close>
 
-locale bfs_invar_tbd = bfs where
+locale bfs_valid_input = bfs where
   Map_update = Map_update and
   P_update = P_update and
   Q_snoc = Q_snoc for
@@ -687,20 +130,47 @@ locale bfs_invar_tbd = bfs where
   assumes invar_G: "G.invar G"
   assumes src_mem_dV: "src \<in> G.dV G"
 
-abbreviation (in bfs_invar_tbd) d :: "'m \<Rightarrow> 'a \<Rightarrow> nat" where
+abbreviation (in bfs) bfs_valid_input' :: "'n \<Rightarrow> 'a \<Rightarrow> bool" where
+  "bfs_valid_input' G src \<equiv>
+   bfs_valid_input
+    Map_empty Map_delete Map_lookup Map_inorder Map_inv
+    Set_empty Set_insert Set_delete Set_isin Set_inorder Set_inv
+    P_empty P_delete P_lookup P_invar
+    Q_empty Q_is_empty Q_head Q_tail Q_invar Q_list
+    Map_update P_update Q_snoc G src"
+
+subsubsection \<open>Loop invariants\<close>
+
+text \<open>
+Unfolding the definition of @{term bfs.bfs}, we see that function @{term bfs.loop} lies at the heart
+of the algorithm. It expects the undirected graph G, the source vertex src in G, as well as the
+current state s, which comprises the queue and parent map, as input. Let us look at the assumptions
+on the queue and parent map. As these are the only two data structures that may change from one
+iteration to the next, these assumptions constitute the loop invariants of @{term bfs.loop}.
+\<close>
+
+text \<open>
+To keep track of progress, the algorithm colors every vertex in G either white, gray, or black. All
+vertices start out white and may later become gray and then black.
+\<close>
+
+abbreviation (in bfs_valid_input) white :: "('q, 'm) state \<Rightarrow> 'a \<Rightarrow> bool" where
+  "white s v \<equiv> \<not> is_discovered src (parent s) v"
+
+abbreviation (in bfs_valid_input) gray :: "('q, 'm) state \<Rightarrow> 'a \<Rightarrow> bool" where
+  "gray s v \<equiv> is_discovered src (parent s) v \<and> v \<in> set (Q_list (queue s))"
+
+abbreviation (in bfs_valid_input) black :: "('q, 'm) state \<Rightarrow> 'a \<Rightarrow> bool" where
+  "black s v \<equiv> is_discovered src (parent s) v \<and> v \<notin> set (Q_list (queue s))"
+
+abbreviation (in bfs) rev_follow :: "'m \<Rightarrow> 'a \<Rightarrow> 'a dpath" where
+  "rev_follow m v \<equiv> rev (parent.follow (P_lookup m) v)"
+
+abbreviation (in bfs_valid_input) d :: "'m \<Rightarrow> 'a \<Rightarrow> nat" where
   "d m v \<equiv> dpath_length (rev_follow m v)"
 
-abbreviation (in bfs_invar_tbd) white :: "('q, 'm) state \<Rightarrow> 'a \<Rightarrow> bool" where
-  "white s v \<equiv> \<not> discovered src (parent s) v"
-
-abbreviation (in bfs_invar_tbd) gray :: "('q, 'm) state \<Rightarrow> 'a \<Rightarrow> bool" where
-  "gray s v \<equiv> discovered src (parent s) v \<and> v \<in> set (Q_list (queue s))"
-
-abbreviation (in bfs_invar_tbd) black :: "('q, 'm) state \<Rightarrow> 'a \<Rightarrow> bool" where
-  "black s v \<equiv> discovered src (parent s) v \<and> v \<notin> set (Q_list (queue s))"
-
 locale bfs_invar =
-  bfs_invar_tbd where P_update = P_update and Q_snoc = Q_snoc +
+  bfs_valid_input where P_update = P_update and Q_snoc = Q_snoc +
   parent "P_lookup (parent s)" for
   P_update :: "'a::linorder \<Rightarrow> 'a \<Rightarrow> 'm \<Rightarrow> 'm" and
   Q_snoc :: "'q \<Rightarrow> 'a \<Rightarrow> 'q" and
@@ -713,27 +183,36 @@ locale bfs_invar =
   assumes not_white_if_parent: "P_lookup (parent s) v = Some u \<Longrightarrow> \<not> white s u"
   assumes black_imp_adjacency_not_white: "\<lbrakk> (u, v) \<in> G.dE G; black s u \<rbrakk> \<Longrightarrow> \<not> white s v"
   assumes queue_sorted_wrt_d: "sorted_wrt (\<lambda>u v. d (parent s) u \<le> d (parent s) v) (Q_list (queue s))"
-  assumes d_last_queue_le: "\<not> Q_is_empty (queue s) \<Longrightarrow> d (parent s) (last (Q_list (queue s))) \<le> d (parent s) (Q_head (queue s)) + 1"
-  assumes d_triangle_inequality: "\<lbrakk> dpath_bet (G.dE G) p u v; \<not> white s u; \<not> white s v \<rbrakk> \<Longrightarrow> d (parent s) v \<le> d (parent s) u + dpath_length p"
+  assumes d_last_queue_le:
+    "\<not> Q_is_empty (queue s) \<Longrightarrow>
+     d (parent s) (last (Q_list (queue s))) \<le> d (parent s) (Q_head (queue s)) + 1"
+  assumes d_triangle_inequality:
+    "\<lbrakk> dpath_bet (G.dE G) p u v; \<not> white s u; \<not> white s v \<rbrakk> \<Longrightarrow>
+     d (parent s) v \<le> d (parent s) u + dpath_length p"
 
-locale bfs_invar_not_DONE = bfs_invar where P_update = P_update and Q_snoc = Q_snoc for
-  P_update :: "'a::linorder \<Rightarrow> 'a \<Rightarrow> 'm \<Rightarrow> 'm" and
-  Q_snoc :: "'q \<Rightarrow> 'a \<Rightarrow> 'q" +
-  assumes not_DONE: "\<not> DONE s"
+text \<open>
+Invariant @{thm bfs_invar.black_imp_adjacency_not_white} says that all vertices adjacent to black
+vertices have been discovered.
+\<close>
 
-locale bfs_invar_DONE = bfs_invar where P_update = P_update and Q_snoc = Q_snoc for
-  P_update :: "'a::linorder \<Rightarrow> 'a \<Rightarrow> 'm \<Rightarrow> 'm" and
-  Q_snoc :: "'q \<Rightarrow> 'a \<Rightarrow> 'q" +
-  assumes DONE: "DONE s"
+text \<open>
+For a vertex $v$ in G, let d v denote the distance from the source src to v induced by the current
+parent map. 
+\<close>
 
-abbreviation (in bfs) bfs_invar_tbd' :: "'n \<Rightarrow> 'a \<Rightarrow> bool" where
-  "bfs_invar_tbd' G src \<equiv>
-   bfs_invar_tbd
-    Map_empty Map_delete Map_lookup Map_inorder Map_inv
-    Set_empty Set_insert Set_delete Set_isin Set_inorder Set_inv
-    P_empty P_delete P_lookup P_invar
-    Q_empty Q_is_empty Q_head Q_tail Q_invar Q_list
-    Map_update P_update Q_snoc G src"
+text \<open>
+Let $v_1,\dots,v_k$ be the content of the current queue, where $v_1$ is the head. Then invariant
+@{thm bfs_invar.queue_sorted_wrt_d} says that $d v_i\leq d v_{i+1}$ for all $i<k$. And invariant
+@{thm bfs_invar.d_last_queue_le} says that $d v_k\leq d v_1 + 1$. That is, the current queue holds at
+most two distinct $d$ values.
+\<close>
+
+text \<open>
+Finally, invariant @{thm bfs_invar.d_triangle_inequality} says that d satisfies a variant of the
+triangle inequality. More specifically, if there is a path in G between two vertices u, v that
+have been discovered by the algorithm, then their d values differ by at most the length of that
+path.
+\<close>
 
 abbreviation (in bfs) bfs_invar' :: "'n \<Rightarrow> 'a \<Rightarrow> ('q, 'm) state \<Rightarrow> bool" where
   "bfs_invar' G src s \<equiv>
@@ -744,321 +223,90 @@ abbreviation (in bfs) bfs_invar' :: "'n \<Rightarrow> 'a \<Rightarrow> ('q, 'm) 
     Q_empty Q_is_empty Q_head Q_tail Q_invar Q_list
     Map_update G src P_update Q_snoc s"
 
-abbreviation (in bfs_invar_tbd) bfs_invar'' :: "('q, 'm) state \<Rightarrow> bool" where
+abbreviation (in bfs_valid_input) bfs_invar'' :: "('q, 'm) state \<Rightarrow> bool" where
   "bfs_invar'' \<equiv> bfs_invar' G src"
 
-abbreviation (in bfs) bfs_invar_not_DONE' :: "'n \<Rightarrow> 'a \<Rightarrow> ('q, 'm) state \<Rightarrow> bool" where
-  "bfs_invar_not_DONE' G src s \<equiv>
-   bfs_invar_not_DONE
-    Map_empty Map_delete Map_lookup Map_inorder Map_inv
-    Set_empty Set_insert Set_delete Set_isin Set_inorder Set_inv
-    P_empty P_delete P_lookup P_invar
-    Q_empty Q_is_empty Q_head Q_tail Q_invar Q_list
-    Map_update G src s P_update Q_snoc"
+text \<open>
+Let us quickly show that the initial configuration of the queue--containing only the source vertex
+src--and parent map--the empty map--satisfies the loop invariants.
+\<close>
 
-abbreviation (in bfs_invar_tbd) bfs_invar_not_DONE'' :: "('q, 'm) state \<Rightarrow> bool" where
-  "bfs_invar_not_DONE'' \<equiv> bfs_invar_not_DONE' G src"
-
-abbreviation (in bfs) bfs_invar_DONE' :: "'n \<Rightarrow> 'a \<Rightarrow> ('q, 'm) state \<Rightarrow> bool" where
-  "bfs_invar_DONE' G src s \<equiv>
-   bfs_invar_DONE
-    Map_empty Map_delete Map_lookup Map_inorder Map_inv
-    Set_empty Set_insert Set_delete Set_isin Set_inorder Set_inv
-    P_empty P_delete P_lookup P_invar
-    Q_empty Q_is_empty Q_head Q_tail Q_invar Q_list
-    Map_update G src s P_update Q_snoc"
-
-abbreviation (in bfs_invar_tbd) bfs_invar_DONE'' :: "('q, 'm) state \<Rightarrow> bool" where
-  "bfs_invar_DONE'' \<equiv> bfs_invar_DONE' G src"
-
-subsection \<open>Convenience Lemmas\<close>
-
-subsubsection \<open>@{term bfs}\<close>
-
-lemma (in bfs) bfs_invar_not_DONE'I:
-  assumes "bfs_invar' G src s"
-  assumes "\<not> DONE s"
-  shows "bfs_invar_not_DONE' G src s"
-  using assms
-  by (simp add: bfs_invar_not_DONE_def bfs_invar_not_DONE_axioms_def)
-
-lemma (in bfs) bfs_invar_DONE'I:
-  assumes "bfs_invar' G src s"
-  assumes "DONE s"
-  shows "bfs_invar_DONE' G src s"
-  using assms
-  by (simp add: bfs_invar_DONE_def bfs_invar_DONE_axioms_def)
-
-lemma (in bfs) rev_follow_non_empty:
-  assumes "Tbd.parent (P_lookup m)"
-  shows "rev_follow m v \<noteq> []"
-  using assms
-  by (auto dest: parent.follow_non_empty)
-
-lemma (in bfs) distinct_rev_follow:
-  assumes "Tbd.parent (P_lookup m)"
-  shows "distinct (rev_follow m v)"
-  unfolding distinct_rev
-  using assms
-  by (intro parent.distinct_follow)
-
-lemma (in bfs) last_rev_follow:
-  assumes "Tbd.parent (P_lookup m)"
-  shows "last (rev_follow m v) = v"
-proof -
-  let ?l = "parent.follow (P_lookup m) v"
-  have "?l = hd ?l # tl ?l"
-    using assms
-    by (intro parent.follow_non_empty hd_Cons_tl[symmetric])
-  hence "hd ?l = v"
-    using assms
-    by (auto dest: parent.follow_ConsD)
-  thus ?thesis
-    using assms parent.follow_non_empty
-    by (fastforce simp add: last_rev)
-qed
-
-subsubsection \<open>@{term bfs_invar_tbd}\<close>
-
-context bfs_invar_tbd
-begin
-sublocale finite_dgraph "G.dE G"
-proof (standard, goal_cases)
-  case 1
-  show ?case
-    using invar_G
-    by (intro G.finite_dE)
-qed
-end
-
-lemma (in bfs_invar_tbd) vertex_color_induct [case_names white gray black]:
-  assumes "white s v \<Longrightarrow> P s v"
-  assumes "gray s v \<Longrightarrow> P s v"
-  assumes "black s v \<Longrightarrow> P s v"
-  shows "P s v"
-  using assms
-  by blast
-
-lemma (in bfs_invar_tbd) src_not_white:
-  shows "\<not> white s src"
-  by (simp add: discovered_def)
-
-subsubsection \<open>@{term bfs_invar}\<close>
-
-lemma (in bfs_invar) distinct_rev_follow:
-  shows "distinct (rev_follow (parent s) v)"
-  using distinct_follow
-  by simp
-
-subsection \<open>Basic Lemmas\<close>
-
-subsubsection \<open>@{term bfs_invar_tbd}\<close>
-
-lemma (in bfs_invar_tbd) parent_imp_d:
-  assumes "Tbd.parent (P_lookup (parent s))"
-  assumes "P_lookup (parent s) v = Some u"
-  shows "d (parent s) v = d (parent s) u + 1"
-proof -
-  have "rev_follow (parent s) v = rev_follow (parent s) u @ [v]"
-    using assms
-    by (simp add: parent.follow_psimps)
-  thus ?thesis
-    using parent.follow_non_empty[OF assms(1)]
-    by (simp add: dpath_length_snoc)
-qed
-
-subsubsection \<open>@{term bfs_invar}\<close>
-
-lemma (in bfs_invar) not_white_imp_dpath_rev_follow:
-  assumes "\<not> white s v"
-  shows "dpath_bet (G.dE G) (rev_follow (parent s) v) src v"
-  using assms
-proof (induct v rule: follow_pinduct)
-  case (1 v)
-  show ?case
-  proof (cases "v = src")
-    case True
-    thus ?thesis
-      using parent_src src_mem_dV
-      by (auto simp add: follow_psimps intro: dpath_bet_reflexive)
-  next
-    case False
-    then obtain u where
-      u: "P_lookup (parent s) v = Some u"
-      using "1.prems"
-      by (auto simp add: discovered_def)
-    hence
-      "follow v = v # follow u"
-      "(u, v) \<in> G.dE G"
-      "\<not> white s u"
-      using not_white_if_parent
-      by (auto simp add: follow_psimps intro: parent_imp_edge)
-    moreover hence "dpath_bet (G.dE G) (rev_follow (parent s) u) src u"
-      using u
-      by (intro "1.hyps")
-    ultimately show ?thesis
-      by (auto intro: dpath_bet_snocI)
-  qed
-qed
-
-lemma (in bfs_invar) hd_rev_follow_eq_src:
-  assumes "\<not> white s v"
-  shows "hd (rev_follow (parent s) v) = src"
-  using assms
-  by (intro hd_of_dpath_bet'[symmetric]) (rule not_white_imp_dpath_rev_follow)
-
-lemma (in bfs_invar) mem_queue_imp_d_ge:
-  assumes "v \<in> set (Q_list (queue s))"
-  shows "d (parent s) (Q_head (queue s)) \<le> d (parent s) v"
-proof (cases "v = Q_head (queue s)")
-  case True
-  thus ?thesis
-    by simp
-next
-  case False
-  have "\<not> Q_is_empty (queue s)"
-    using invar_queue assms
-    by (auto simp add: Q.is_empty)
-  moreover hence "Q_head (queue s) = hd (Q_list (queue s))"
-    using invar_queue Q.list_head
-    by (simp add: Q.is_empty)
-  ultimately show ?thesis
-    using queue_sorted_wrt_d assms False sorted_wrt_imp_hd
-    by fastforce
-qed
-
-lemma (in bfs_invar) mem_queue_imp_d_le:
-  assumes "v \<in> set (Q_list (queue s))"
-  shows "d (parent s) v \<le> d (parent s) (last (Q_list (queue s)))"
-proof (cases "v = last (Q_list (queue s))")
-  case True
-  thus ?thesis
-    by simp
-next
-  case False
-  have "\<not> Q_is_empty (queue s)"
-    using invar_queue assms
-    by (auto simp add: Q.is_empty)
-  thus ?thesis
-    using queue_sorted_wrt_d assms False sorted_wrt_imp_last
-    by fastforce
-qed
-
-lemma (in bfs_invar) d_triangle_inequality_edge:
-  assumes "(u, v) \<in> G.dE G"
-  assumes "\<not> white s u"
-  assumes "\<not> white s v"
-  shows "d (parent s) v \<le> d (parent s) u + 1"
-proof -
-  have "dpath_bet (G.dE G) [u, v] u v"
-    using assms(1)
-    by (intro edges_are_dpath_bet)
-  thus ?thesis
-    using assms(2, 3)
-    using d_triangle_inequality
-    by fastforce
-qed
-
-subsection \<open>@{term bfs.init}\<close>
-
-subsubsection \<open>\<close>
-
-lemma (in bfs_invar_tbd) follow_invar'_parent_init:
-  shows "follow_invar' (P_lookup (parent (init src)))"
+lemma (in bfs_valid_input) follow_invar_parent_init:
+  shows "follow_invar (P_lookup (parent (init src)))"
   using wf_empty
-  by (simp add: init_def P.map_empty follow_invar'_def)
+  by (simp add: init_def P.map_empty follow_invar_def)
 
-subsubsection \<open>@{thm bfs_invar.invar_queue}\<close>
-
-lemma (in bfs_invar_tbd) invar_queue_init:
+lemma (in bfs_valid_input) invar_queue_init:
   shows "Q_invar (queue (init src))"
   using Q.invar_empty
   by (auto simp add: init_def intro: Q.invar_snoc)
 
-subsubsection \<open>@{thm bfs_invar.invar_parent}\<close>
-
-lemma (in bfs_invar_tbd) invar_parent_init:
+lemma (in bfs_valid_input) invar_parent_init:
   shows "P_invar (parent (init src))"
   using P.invar_empty
   by (simp add: init_def)
 
-subsubsection \<open>@{thm bfs_invar.parent_src}\<close>
-
-lemma (in bfs_invar_tbd) parent_src_init:
+lemma (in bfs_valid_input) parent_src_init:
   shows "P_lookup (parent (init src)) src = None"
   by (simp add: init_def P.map_empty)
 
-subsubsection \<open>@{thm bfs_invar.parent_imp_edge}\<close>
-
-lemma (in bfs_invar_tbd) parent_imp_edge_init:
+lemma (in bfs_valid_input) parent_imp_edge_init:
   assumes "P_lookup (parent (init src)) v = Some u"
   shows "(u, v) \<in> G.dE G"
   using assms
   by (simp add: init_def P.map_empty)
 
-subsubsection \<open>@{thm bfs_invar.not_white_if_mem_queue}\<close>
-
-lemma (in bfs_invar_tbd) not_white_if_mem_queue_init:
+lemma (in bfs_valid_input) not_white_if_mem_queue_init:
   assumes "v \<in> set (Q_list (queue (init src)))"
   shows "\<not> white (init src) v"
   using assms Q.invar_empty
-  by (simp add: init_def Q.list_snoc Q.list_empty discovered_def)
+  by (simp add: init_def Q.list_snoc Q.list_empty is_discovered_def)
 
-subsubsection \<open>@{thm bfs_invar.not_white_if_parent}\<close>
-
-lemma (in bfs_invar_tbd) not_white_if_parent_init:
+lemma (in bfs_valid_input) not_white_if_parent_init:
   assumes "P_lookup (parent (init src)) v = Some u"
   shows "\<not> white (init src) u"
   using assms
   by (simp add: init_def P.map_empty)
 
-subsubsection \<open>@{thm bfs_invar.black_imp_adjacency_not_white}\<close>
-
-lemma (in bfs_invar_tbd) black_imp_adjacency_not_white_init:
+lemma (in bfs_valid_input) black_imp_adjacency_not_white_init:
   assumes "black (init src) u"
   assumes "(u, v) \<in> G.dE G"
   shows "\<not> white s v"
 proof -
   have "u = src"
     using assms(1)
-    by (simp add: discovered_def init_def P.map_empty)
+    by (simp add: is_discovered_def init_def P.map_empty)
   thus ?thesis
     using assms(1) Q.invar_empty
     by (simp add: init_def Q.list_snoc)
 qed
 
-subsubsection \<open>@{thm bfs_invar.queue_sorted_wrt_d}\<close>
-
-lemma (in bfs_invar_tbd) queue_sorted_wrt_d_init:
+lemma (in bfs_valid_input) queue_sorted_wrt_d_init:
   shows "sorted_wrt (\<lambda>u v. d (parent (init src)) u \<le> d (parent (init src)) v) (Q_list (queue (init src)))"
   using Q.invar_empty
   by (simp add: init_def Q.list_snoc Q.list_empty)
 
-subsubsection \<open>@{thm bfs_invar.d_last_queue_le}\<close>
-
-lemma (in bfs_invar_tbd) d_last_queue_le_init:
+lemma (in bfs_valid_input) d_last_queue_le_init:
   assumes "\<not> Q_is_empty (queue (init src))"
-  shows "d (parent (init src)) (last (Q_list (queue (init src)))) \<le> d (parent (init src)) (Q_head (queue (init src))) + 1"
+  shows
+    "d (parent (init src)) (last (Q_list (queue (init src)))) \<le>
+     d (parent (init src)) (Q_head (queue (init src))) + 1"
   using Q.invar_empty invar_queue_init
   by (simp add: init_def Q.list_snoc Q.list_empty Q.list_head)
 
-subsubsection \<open>@{thm bfs_invar.d_triangle_inequality}\<close>
-
-lemma (in bfs_invar_tbd) d_triangle_inequality_init:
+lemma (in bfs_valid_input) d_triangle_inequality_init:
   assumes "dpath_bet (G.dE G) p u v"
   assumes "\<not> white (init src) u"
   assumes "\<not> white (init src) v"
   shows "d (parent (init src)) v \<le> d (parent (init src)) u + dpath_length p"
   using assms
-  by (simp add: discovered_def init_def P.map_empty)
+  by (simp add: is_discovered_def init_def P.map_empty)
 
-subsubsection \<open>\<close>
-
-lemma (in bfs_invar_tbd) bfs_invar_init:
+lemma (in bfs_valid_input) bfs_invar_init:
   shows "bfs_invar'' (init src)"
 proof (standard, goal_cases)
   case 1
-  show ?case using follow_invar'_parent_init .
+  show ?case using follow_invar_parent_init .
 next
   case 2
   show ?case using invar_queue_init .
@@ -1091,17 +339,225 @@ next
   thus ?case by (intro d_triangle_inequality_init)
 qed
 
-subsection \<open>@{term bfs.fold}\<close>
+text \<open>
+Let us now show that the loop invariants are maintained, that is, if they are satisfied at the start
+of an iteration, then they also will be satisfied at the end.
+\<close>
 
-subsubsection \<open>Convenience Lemmas\<close>
+text \<open>For this, let us first look at how the different subroutines change the queue and parent map.\<close>
 
-lemma (in bfs_invar_not_DONE) list_queue_fold_cong:
+text \<open>How does @{term bfs.discover} change the queue and parent map?\<close>
+
+lemma (in bfs) queue_discover_cong [simp]:
+  shows "queue (discover u v s) = Q_snoc (queue s) v"
+  by (simp add: discover_def)
+
+lemma (in bfs) parent_discover_cong [simp]:
+  shows "parent (discover u v s) = P_update v u (parent s)"
+  by (simp add: discover_def)
+
+text \<open>How does @{term bfs.traverse_edge} change the queue and parent map?\<close>
+
+lemma (in bfs) queue_traverse_edge_cong:
+  shows "queue (traverse_edge src u v s) = (if \<not> is_discovered src (parent s) v then Q_snoc (queue s) v else queue s)"
+  by (simp add: traverse_edge_def)
+
+lemma (in bfs) invar_queue_traverse_edge:
+  assumes "Q_invar (queue s)"
+  shows "Q_invar (queue (traverse_edge src u v s))"
+  using assms Q.invar_snoc
+  by (simp add: queue_traverse_edge_cong)
+
+lemma (in bfs) list_queue_traverse_edge_cong:
+  assumes "Q_invar (queue s)"
+  shows
+    "Q_list (queue (traverse_edge src u v s)) =
+     Q_list (queue s) @ (if \<not> is_discovered src (parent s) v then [v] else [])"
+  using assms
+  by (simp add: queue_traverse_edge_cong Q.list_snoc)
+
+lemma (in bfs) invar_parent_traverse_edge:
+  assumes "P_invar (parent s)"
+  shows "P_invar (parent (traverse_edge src u v s))"
+  using assms P.invar_update
+  by (simp add: traverse_edge_def)
+
+lemma (in bfs) lookup_parent_traverse_edge_cong:
+  assumes "P_invar (parent s)"
+  shows
+    "P_lookup (parent (traverse_edge src u v s)) =
+     override_on
+      (P_lookup (parent s))
+      (\<lambda>_. Some u)
+      (if \<not> is_discovered src (parent s) v then {v} else {})"
+  using assms
+  by (simp add: traverse_edge_def P.map_update override_on_insert')
+
+lemma (in bfs) T_traverse_edge_cong:
+  assumes "P_invar (parent s)"
+  shows "T (parent (traverse_edge src u v s)) = T (parent s) \<union> (if \<not> is_discovered src (parent s) v then {(u, v)} else {})"
+  using assms
+  by (auto simp add: lookup_parent_traverse_edge_cong override_on_def is_discovered_def)
+
+text \<open>How does @{term bfs.fold} change the queue and parent map?\<close>
+
+lemma (in bfs) list_queue_fold_cong_aux:
+  assumes "P_invar (parent s)"
+  assumes "distinct (v # vs)"
+  shows "filter (Not \<circ> is_discovered src (parent (traverse_edge src u v s))) vs = filter (Not \<circ> is_discovered src (parent s)) vs"
+proof (rule filter_cong)
+  fix w
+  assume "w \<in> set vs"
+  hence "is_discovered src (parent (traverse_edge src u v s)) w = is_discovered src (parent s) w"
+    using assms
+    by (auto simp add: is_discovered_def lookup_parent_traverse_edge_cong override_on_insert')
+  thus "(Not \<circ> is_discovered src (parent (traverse_edge src u v s))) w = (Not \<circ> is_discovered src (parent s)) w"
+    by simp
+qed simp
+
+lemma (in bfs) list_queue_fold_cong:
+  assumes "Q_invar (queue s)"
+  assumes "P_invar (parent s)"
+  assumes "distinct l"
+  shows
+    "Q_list (queue (List.fold (traverse_edge src u) l s)) =
+     Q_list (queue s) @ filter (Not \<circ> is_discovered src (parent s)) l"
+  using assms
+proof (induct l arbitrary: s)
+  case Nil
+  thus ?case
+    by simp
+next
+  case (Cons v vs)
+  have
+    "Q_list (queue (List.fold (traverse_edge src u) (v # vs) s)) =
+     Q_list (queue (List.fold (traverse_edge src u) vs (traverse_edge src u v s)))"
+    by simp
+  also have
+    "... =
+     Q_list (queue (traverse_edge src u v s)) @
+     filter (Not \<circ> is_discovered src (parent (traverse_edge src u v s))) vs"
+    using Cons.prems
+    by (auto intro: invar_queue_traverse_edge invar_parent_traverse_edge Cons.hyps)
+  also have
+    "... =
+     Q_list (queue s) @
+     (if \<not> is_discovered src (parent s) v then [v] else []) @
+     filter (Not \<circ> is_discovered src (parent (traverse_edge src u v s))) vs"
+    using Cons.prems(1)
+    by (simp add: list_queue_traverse_edge_cong)
+  also have
+    "... =
+     Q_list (queue s) @
+     (if \<not> is_discovered src (parent s) v then [v] else []) @
+     filter (Not \<circ> is_discovered src (parent s)) vs"
+    using Cons.prems(2, 3)
+    by (simp add: list_queue_fold_cong_aux)
+  also have "... = Q_list (queue s) @ filter (Not \<circ> is_discovered src (parent s)) (v # vs)"
+    by simp
+  finally show ?case
+    .
+qed
+
+lemma (in bfs) invar_tail:
+  assumes "Q_invar (queue s)"
+  assumes "\<not> DONE s"
+  shows "Q_invar (queue (s\<lparr>queue := Q_tail (queue s)\<rparr>))"
+  using assms Q.invar_tail
+  by (simp add: DONE_def Q.is_empty)
+
+lemma (in bfs) list_queue_fold_cong_2:
+  assumes "G.invar G"
+  assumes "Q_invar (queue s)"
+  assumes "P_invar (parent s)"
+  assumes "\<not> DONE s"
   shows
     "Q_list (queue (fold G src s)) =
      Q_list (Q_tail (queue s)) @
-     filter (Not \<circ> discovered src (parent s)) (G.adjacency G (Q_head (queue s)))"
-  using invar_G invar_queue invar_parent not_DONE
-  by (intro list_queue_fold_cong_2)
+     filter (Not \<circ> is_discovered src (parent s)) (G.adjacency_list G (Q_head (queue s)))"
+proof -
+  have
+    "Q_list (queue (fold G src s)) =
+     Q_list (queue (s\<lparr>queue := Q_tail (queue s)\<rparr>)) @
+     filter
+      (Not \<circ> is_discovered src (parent (s\<lparr>queue := Q_tail (queue s)\<rparr>)))
+      (G.adjacency_list G (Q_head (queue s)))"
+    using assms
+    by (intro invar_tail G.distinct_adjacency_list list_queue_fold_cong) simp+
+  thus ?thesis
+    unfolding comp_apply
+    by (simp add: is_discovered_def)
+qed
+
+lemma (in bfs) lookup_parent_fold_cong:
+  assumes "P_invar (parent s)"
+  assumes "distinct l"
+  shows
+    "P_lookup (parent (List.fold (traverse_edge src u) l s)) =
+     override_on
+      (P_lookup (parent s))
+      (\<lambda>_. Some u)
+      (set (filter (Not \<circ> is_discovered src (parent s)) l))"
+  using assms
+proof (induct l arbitrary: s)
+  case Nil
+  thus ?case
+    by simp
+next
+  case (Cons v vs)
+  have
+    "P_lookup (parent (List.fold (traverse_edge src u) (v # vs) s)) =
+     P_lookup (parent (List.fold (traverse_edge src u) vs (traverse_edge src u v s)))"
+    by simp
+  also have
+    "... =
+     override_on
+      (P_lookup (parent (traverse_edge src u v s)))
+      (\<lambda>_. Some u)
+      (set (filter (Not \<circ> is_discovered src (parent (traverse_edge src u v s))) vs))"
+    using Cons.prems
+    by (fastforce intro: invar_parent_traverse_edge Cons.hyps)
+  also have
+    "... =
+     override_on
+      (override_on (P_lookup (parent s)) (\<lambda>_. Some u) (if \<not> is_discovered src (parent s) v then {v} else {}))
+      (\<lambda>_. Some u)
+      (set (filter (Not \<circ> is_discovered src (parent (traverse_edge src u v s))) vs))"
+    using Cons.prems(1)
+    by (simp add: lookup_parent_traverse_edge_cong)
+  also have
+    "... =
+     override_on
+      (override_on (P_lookup (parent s)) (\<lambda>_. Some u) (if \<not> is_discovered src (parent s) v then {v} else {}))
+      (\<lambda>_. Some u)
+      (set (filter (Not \<circ> is_discovered src (parent s)) vs))"
+    using Cons.prems
+    by (simp add: list_queue_fold_cong_aux)
+  finally show ?case
+    by (simp add: override_on_insert')
+qed
+
+lemma (in bfs) lookup_parent_fold_cong_2:
+  assumes "G.invar G"
+  assumes "P_invar (parent s)"
+  shows
+    "P_lookup (parent (fold G src s)) =
+     override_on
+      (P_lookup (parent s))
+      (\<lambda>_. Some (Q_head (queue s)))
+      (set (filter (Not \<circ> is_discovered src (parent s)) (G.adjacency_list G (Q_head (queue s)))))"
+proof -
+  have
+    "P_lookup (parent (fold G src s)) =
+     override_on
+      (P_lookup (parent (s\<lparr>queue := Q_tail (queue s)\<rparr>)))
+      (\<lambda>_. Some (Q_head (queue s)))
+      (set (filter (Not \<circ> is_discovered src (parent (s\<lparr>queue := Q_tail (queue s)\<rparr>))) (G.adjacency_list G (Q_head (queue s)))))"
+    using assms
+    by (intro G.distinct_adjacency_list lookup_parent_fold_cong) simp+
+  thus ?thesis
+    by (simp add: is_discovered_def)
+qed
 
 lemma (in bfs_invar) lookup_parent_fold_cong:
   shows
@@ -1109,17 +565,113 @@ lemma (in bfs_invar) lookup_parent_fold_cong:
      override_on
       (P_lookup (parent s))
       (\<lambda>_. Some (Q_head (queue s)))
-      (set (filter (Not \<circ> discovered src (parent s)) (G.adjacency G (Q_head (queue s)))))"
+      (set (filter (Not \<circ> is_discovered src (parent s)) (G.adjacency_list G (Q_head (queue s)))))"
   using invar_G invar_parent
   by (intro lookup_parent_fold_cong_2)
+
+lemma (in bfs) T_fold_cong_aux:
+  assumes "P_invar (parent s)"
+  assumes "distinct (v # vs)"
+  shows "w \<in> set vs \<and> \<not> is_discovered src (parent (traverse_edge src u v s)) w \<longleftrightarrow> w \<in> set vs \<and> \<not> is_discovered src (parent s) w"
+  using assms
+  by (auto simp add: is_discovered_def lookup_parent_traverse_edge_cong override_on_def)
+
+lemma (in bfs) T_fold_cong:
+  assumes "P_invar (parent s)"
+  assumes "distinct l"
+  shows "T (parent (List.fold (traverse_edge src u) l s)) = T (parent s) \<union> {(u, v) |v. v \<in> set l \<and> \<not> is_discovered src (parent s) v}"
+  using assms
+proof (induct l arbitrary: s)
+  case Nil
+  thus ?case
+    by auto
+next
+  case (Cons v vs)
+  have
+    "T (parent (List.fold (traverse_edge src u) (v # vs) s)) =
+     T (parent (List.fold (traverse_edge src u) vs (traverse_edge src u v s)))"
+    by simp
+  also have
+    "... =
+     T (parent (traverse_edge src u v s)) \<union>
+     {(u, w) |w. w \<in> set vs \<and> \<not> is_discovered src (parent (traverse_edge src u v s)) w}"
+    using Cons.prems
+    by (intro invar_parent_traverse_edge Cons.hyps) simp+
+  also have
+    "... =
+     T (parent s) \<union>
+     (if \<not> is_discovered src (parent s) v then {(u, v)} else {}) \<union>
+     {(u, w) |w. w \<in> set vs \<and> \<not> is_discovered src (parent (traverse_edge src u v s)) w}"
+    unfolding T_traverse_edge_cong[OF Cons.prems(1)]
+    by blast
+  also have
+    "... =
+     T (parent s) \<union>
+     (if \<not> is_discovered src (parent s) v then {(u, v)} else {}) \<union>
+     {(u, w) |w. w \<in> set vs \<and> \<not> is_discovered src (parent s) w}"
+    using Cons.prems
+    by (simp add: T_fold_cong_aux)
+  also have "... = T (parent s) \<union> {(u, w) |w. w \<in> set (v # vs) \<and> \<not> is_discovered src (parent s) w}"
+    by force
+  finally show ?case
+    .
+qed
+
+lemma (in bfs) T_fold_cong_2:
+  assumes "G.invar G"
+  assumes "P_invar (parent s)"
+  shows
+    "T (parent (fold G src s)) =
+     T (parent s) \<union>
+     {(Q_head (queue s), v) |v. v \<in> set (G.adjacency_list G (Q_head (queue s))) \<and> \<not> is_discovered src (parent s) v}"
+proof -
+  have
+    "T (parent (fold G src s)) =
+     T (parent (s\<lparr>queue := Q_tail (queue s)\<rparr>)) \<union>
+     {(Q_head (queue s), v) |v.
+      v \<in> set (G.adjacency_list G (Q_head (queue s))) \<and>
+      \<not> is_discovered src (parent (s\<lparr>queue := Q_tail (queue s)\<rparr>)) v}"
+    using assms
+    by (intro G.distinct_adjacency_list T_fold_cong) simp+
+  thus ?thesis
+    by (simp add: is_discovered_def)
+qed
 
 lemma (in bfs_invar) T_fold_cong:
   shows
     "T (parent (fold G src s)) =
      T (parent s) \<union>
-     {(Q_head (queue s), v) |v. v \<in> set (G.adjacency G (Q_head (queue s))) \<and> \<not> discovered src (parent s) v}"
+     {(Q_head (queue s), v) |v. v \<in> set (G.adjacency_list G (Q_head (queue s))) \<and> \<not> is_discovered src (parent s) v}"
   using invar_G invar_parent
   by (intro T_fold_cong_2)
+
+text \<open>We are now ready to prove that the variants are maintained.\<close>
+
+locale bfs_invar_not_DONE = bfs_invar where P_update = P_update and Q_snoc = Q_snoc for
+  P_update :: "'a::linorder \<Rightarrow> 'a \<Rightarrow> 'm \<Rightarrow> 'm" and
+  Q_snoc :: "'q \<Rightarrow> 'a \<Rightarrow> 'q" +
+assumes not_DONE: "\<not> DONE s"
+
+abbreviation (in bfs) bfs_invar_not_DONE' :: "'n \<Rightarrow> 'a \<Rightarrow> ('q, 'm) state \<Rightarrow> bool" where
+  "bfs_invar_not_DONE' G src s \<equiv>
+   bfs_invar_not_DONE
+    Map_empty Map_delete Map_lookup Map_inorder Map_inv
+    Set_empty Set_insert Set_delete Set_isin Set_inorder Set_inv
+    P_empty P_delete P_lookup P_invar
+    Q_empty Q_is_empty Q_head Q_tail Q_invar Q_list
+    Map_update G src s P_update Q_snoc"
+
+abbreviation (in bfs_valid_input) bfs_invar_not_DONE'' :: "('q, 'm) state \<Rightarrow> bool" where
+  "bfs_invar_not_DONE'' \<equiv> bfs_invar_not_DONE' G src"
+
+text \<open>We start with the first invariant.\<close>
+
+lemma (in bfs) list_queue_non_empty:
+  assumes "Q_invar (queue s)"
+  assumes "\<not> DONE s"
+  shows "Q_list (queue s) \<noteq> []"
+  using assms
+  by (simp add: DONE_def Q.is_empty)
 
 lemma (in bfs_invar_not_DONE) list_queue_non_empty:
   shows "Q_list (queue s) \<noteq> []"
@@ -1136,18 +688,16 @@ lemma (in bfs_invar_not_DONE) not_white_head_queue:
   using head_queue_mem_queue
   by (intro not_white_if_mem_queue)
 
-subsubsection \<open>\<close>
-
-lemma (in bfs_invar_not_DONE) follow_invar'_parent_fold:
-  shows "follow_invar' (P_lookup (parent (fold G src s)))"
-  unfolding follow_invar'_def T_fold_cong
+lemma (in bfs_invar_not_DONE) follow_invar_parent_fold:
+  shows "follow_invar (P_lookup (parent (fold G src s)))"
+  unfolding follow_invar_def T_fold_cong
 proof (rule wf_Un)
   let ?r =
     "{(Q_head (queue s), v) |v.
-      v \<in> set (G.adjacency G (Q_head (queue s))) \<and> \<not> discovered src (parent s) v}"
+      v \<in> set (G.adjacency_list G (Q_head (queue s))) \<and> \<not> is_discovered src (parent s) v}"
   show "wf (T (parent s))"
-    using follow_invar'
-    by (simp add: follow_invar'_def)
+    using follow_invar
+    by (simp add: follow_invar_def)
   have "\<not> white s (Q_head (queue s))"
     using not_white_head_queue
     .
@@ -1158,38 +708,155 @@ proof (rule wf_Un)
     by auto
 qed
 
-lemma (in bfs_invar_not_DONE) parent_fold:
-  shows "Tbd.parent (P_lookup (parent (fold G src s)))"
-proof (standard, goal_cases)
-  case 1
-  show ?case
-    by (intro follow_invar'_parent_fold)
-qed
+text \<open>Then the second invariant, @{thm bfs_invar.invar_queue}.\<close>
 
-subsubsection \<open>@{thm bfs_invar.invar_queue}\<close>
+lemma (in bfs) invar_queue_fold:
+  assumes "Q_invar (queue s)"
+  assumes "distinct l"
+  shows "Q_invar (queue (List.fold (traverse_edge src u) l s))"
+  using assms
+  by (induct l arbitrary: s) (simp_all add: invar_queue_traverse_edge)
+
+lemma (in bfs) invar_queue_fold_2:
+  assumes "G.invar G"
+  assumes "Q_invar (queue s)"
+  assumes "\<not> DONE s"
+  shows "Q_invar (queue (fold G src s))"
+  using assms
+  by (auto intro: G.distinct_adjacency_list invar_tail invar_queue_fold)
 
 lemma (in bfs_invar_not_DONE) invar_queue_fold:
   shows "Q_invar (queue (fold G src s))"
   using invar_G invar_queue not_DONE
   by (intro invar_queue_fold_2)
 
-subsubsection \<open>@{thm bfs_invar.invar_parent}\<close>
+text \<open>Then the third invariant, @{thm bfs_invar.invar_parent}.\<close>
+
+lemma (in bfs) invar_parent_fold:
+  assumes "P_invar (parent s)"
+  assumes "distinct l"
+  shows "P_invar (parent (List.fold (traverse_edge src u) l s))"
+  using assms
+  by (induct l arbitrary: s) (simp_all add: invar_parent_traverse_edge)
+
+lemma (in bfs) invar_parent_fold_2:
+  assumes "G.invar G"
+  assumes "P_invar (parent s)"
+  shows "P_invar (parent (fold G src s))"
+  using assms
+  by (intro G.distinct_adjacency_list invar_parent_fold) simp+
 
 lemma (in bfs_invar) invar_parent_fold:
   shows "P_invar (parent (fold G src s))"
   using invar_G invar_parent
   by (intro invar_parent_fold_2)
 
-subsubsection \<open>@{thm bfs_invar.parent_src}\<close>
+text \<open>Then the fourth invariant, @{thm bfs_invar.parent_src}.\<close>
+
+lemma (in bfs_valid_input) src_not_white:
+  shows "\<not> white s src"
+  by (simp add: is_discovered_def)
 
 lemma (in bfs_invar) parent_src_fold:
   shows "P_lookup (parent (fold G src s)) src = None"
   using invar_G invar_parent src_not_white
   by (simp add: lookup_parent_fold_cong_2 parent_src)
 
-subsubsection \<open>Basic Lemmas\<close>
+text \<open>Then the fifth invariant, @{thm bfs_invar.parent_imp_edge}.\<close>
 
-lemma (in bfs_invar_not_DONE) head_queueI:
+lemma (in bfs_invar) head_queueI:
+  assumes "P_lookup (parent s) v \<noteq> Some u"
+  assumes "P_lookup (parent (fold G src s)) v = Some u"
+  shows "u = Q_head (queue s)"
+  using assms
+  by (simp add: lookup_parent_fold_cong override_on_def split: if_splits(2))
+
+lemma (in bfs_invar_not_DONE) parent_imp_edge_fold:
+  assumes "P_lookup (parent (fold G src s)) v = Some u"
+  shows "(u, v) \<in> G.dE G"
+proof (cases "P_lookup (parent s) v = Some u")
+  case True
+  thus ?thesis
+    by (intro parent_imp_edge)
+next
+  case False
+  thus ?thesis
+    using assms head_queueI G.mem_adjacency_iff_edge
+    by (fastforce simp add: lookup_parent_fold_cong)
+qed
+
+text \<open>Then the sixth invariant, @{thm bfs_invar.not_white_if_mem_queue}.\<close>
+
+lemma (in bfs_invar) not_white_imp_not_white_fold:
+  assumes "\<not> white s v"
+  shows "\<not> white (fold G src s) v"
+  using assms
+  by (auto simp add: is_discovered_def lookup_parent_fold_cong)
+
+lemma (in bfs_invar_not_DONE) list_queue_fold_cong:
+  shows
+    "Q_list (queue (fold G src s)) =
+     Q_list (Q_tail (queue s)) @
+     filter (Not \<circ> is_discovered src (parent s)) (G.adjacency_list G (Q_head (queue s)))"
+  using invar_G invar_queue invar_parent not_DONE
+  by (intro list_queue_fold_cong_2)
+
+lemma (in bfs_invar_not_DONE) not_white_if_mem_queue_fold:
+  assumes "v \<in> set (Q_list (queue (fold G src s)))"
+  shows "\<not> white (fold G src s) v"
+proof (cases "v \<in> set (Q_list (queue s))")
+  case True
+  thus ?thesis
+    by (intro not_white_if_mem_queue not_white_imp_not_white_fold)
+next
+  case False
+  hence "v \<notin> set (Q_list (Q_tail (queue s)))"
+    using invar_queue list_queue_non_empty
+    by (auto simp add: Q.list_tail intro: list.set_sel(2))
+  hence "v \<in> set (G.adjacency_list G (Q_head (queue s))) \<and> \<not> is_discovered src (parent s) v"
+    using assms
+    by (simp add: list_queue_fold_cong)
+  thus ?thesis
+    using assms
+    by (fastforce simp add: is_discovered_def lookup_parent_fold_cong)
+qed
+
+text \<open>Then the seventh invariant, @{thm bfs_invar.not_white_if_parent}.\<close>
+
+lemma (in bfs_invar_not_DONE) not_white_if_parent_fold:
+  assumes "P_lookup (parent (fold G src s)) v = Some u"
+  shows "\<not> white (fold G src s) u"
+proof (cases "P_lookup (parent s) v = Some u")
+  case True
+  thus ?thesis
+    by (intro not_white_if_parent not_white_imp_not_white_fold)
+next
+  case False
+  hence "u = Q_head (queue s)"
+    using assms
+    by (intro head_queueI)
+  thus ?thesis
+    using not_white_head_queue
+    by (intro not_white_imp_not_white_fold) simp
+qed
+
+text \<open>Then the eighth invariant, @{thm bfs_invar.black_imp_adjacency_not_white}.\<close>
+
+lemma (in bfs_valid_input) vertex_color_induct [case_names white gray black]:
+  assumes "white s v \<Longrightarrow> P s v"
+  assumes "gray s v \<Longrightarrow> P s v"
+  assumes "black s v \<Longrightarrow> P s v"
+  shows "P s v"
+  using assms
+  by blast
+
+lemma (in bfs_invar_not_DONE) whiteD:
+  assumes "white s v"
+  shows "\<not> black (fold G src s) v"
+  using assms
+  by (auto simp add: is_discovered_def lookup_parent_fold_cong list_queue_fold_cong)
+
+lemma (in bfs_invar_not_DONE) head_queueI_2:
   assumes "v \<in> set (Q_list (queue s))"
   assumes "v \<notin> set (Q_list (queue (fold G src s)))"
   shows "v = Q_head (queue s)"
@@ -1202,24 +869,39 @@ proof -
     by (simp add: list_queue_fold_cong)
 qed
 
-lemma (in bfs_invar) head_queueI_2:
-  assumes "P_lookup (parent s) v \<noteq> Some u"
-  assumes "P_lookup (parent (fold G src s)) v = Some u"
-  shows "u = Q_head (queue s)"
-  using assms
-  by (simp add: lookup_parent_fold_cong override_on_def split: if_splits(2))
-
-lemma (in bfs_invar_not_DONE) whiteD:
-  assumes "white s v"
-  shows "\<not> black (fold G src s) v"
-  using assms
-  by (auto simp add: discovered_def lookup_parent_fold_cong list_queue_fold_cong)
-
-lemma (in bfs_invar) not_white_imp_not_white_fold:
-  assumes "\<not> white s v"
+lemma (in bfs_invar_not_DONE) black_imp_adjacency_not_white_fold:
+  assumes "black (fold G src s) u"
+  assumes "(u, v) \<in> G.dE G"
   shows "\<not> white (fold G src s) v"
-  using assms
-  by (auto simp add: discovered_def lookup_parent_fold_cong)
+proof (induct s u rule: vertex_color_induct)
+  case white
+  thus ?case
+    using assms(1) whiteD
+    by blast
+next
+  case gray
+  hence "u = Q_head (queue s)"
+    using assms(1)
+    by (intro head_queueI_2) simp+
+  thus ?case
+    using assms(2)
+    by (simp add: is_discovered_def lookup_parent_fold_cong override_on_def G.mem_adjacency_iff_edge)
+next
+  case black
+  thus ?case
+    using assms(2)
+    by (intro black_imp_adjacency_not_white not_white_imp_not_white_fold)
+qed
+
+text \<open>Then the ninth invariant, @{thm bfs_invar.queue_sorted_wrt_d}.\<close>
+
+lemma (in bfs_invar_not_DONE) parent_fold:
+  shows "Parent_Relation.parent (P_lookup (parent (fold G src s)))"
+proof (standard, goal_cases)
+  case 1
+  show ?case
+    by (intro follow_invar_parent_fold)
+qed
 
 lemma (in bfs_invar) not_white_imp_lookup_parent_fold_eq_lookup_parent:
   assumes "\<not> white s v"
@@ -1254,7 +936,7 @@ proof (induct v rule: follow_pinduct)
       "P_lookup (parent s) v = Some u"
       "\<not> white s u"
       using "1.prems"(1) not_white_if_parent
-      by (auto simp add: discovered_def)
+      by (auto simp add: is_discovered_def)
     moreover hence "P_lookup (parent (fold G src s)) v = Some u"
       using "1.prems"
       by (simp add: not_white_imp_lookup_parent_fold_eq_lookup_parent)
@@ -1265,17 +947,29 @@ proof (induct v rule: follow_pinduct)
       by (simp_all add: follow_psimps parent.follow_psimps)
     thus ?thesis
       using u
-      by (simp add: "1.hyps"(2))
+      by (simp add: "1.hyps")
   qed
 qed
 
-lemmas (in bfs_invar_not_DONE) not_whiteD =
-  not_white_imp_not_white_fold
-  not_white_imp_lookup_parent_fold_eq_lookup_parent
-  not_white_imp_rev_follow_fold_eq_rev_follow
+lemma (in bfs_invar) mem_queue_imp_d_le:
+  assumes "v \<in> set (Q_list (queue s))"
+  shows "d (parent s) v \<le> d (parent s) (last (Q_list (queue s)))"
+proof (cases "v = last (Q_list (queue s))")
+  case True
+  thus ?thesis
+    by simp
+next
+  case False
+  have "\<not> Q_is_empty (queue s)"
+    using invar_queue assms
+    by (auto simp add: Q.is_empty)
+  thus ?thesis
+    using queue_sorted_wrt_d assms False sorted_wrt_imp_last
+    by fastforce
+qed
 
 lemma (in bfs_invar_not_DONE) mem_filterD:
-  assumes "v \<in> set (filter (Not \<circ> discovered src (parent s)) (G.adjacency G (Q_head (queue s))))"
+  assumes "v \<in> set (filter (Not \<circ> is_discovered src (parent s)) (G.adjacency_list G (Q_head (queue s))))"
   shows
     "d (parent (fold G src s)) v = d (parent (fold G src s)) (Q_head (queue s)) + 1"
     "d (parent (fold G src s)) (last (Q_list (queue s))) \<le> d (parent (fold G src s)) v"
@@ -1293,13 +987,13 @@ proof -
 
   have "d (parent (fold G src s)) (last (Q_list (queue s))) = d (parent s) (last (Q_list (queue s)))"
     using assms list_queue_non_empty not_white_if_mem_queue
-    by (simp add: not_whiteD(3))
+    by (simp add: not_white_imp_rev_follow_fold_eq_rev_follow)
   also have "... \<le> d (parent s) ?u + 1"
     using not_DONE d_last_queue_le
     by (simp add: DONE_def)
   also have "... = d (parent (fold G src s)) ?u + 1"
     using assms not_white_head_queue
-    by (simp add: not_whiteD(3))
+    by (simp add: not_white_imp_rev_follow_fold_eq_rev_follow)
   also have "... = d (parent (fold G src s)) v"
     unfolding d_eq
     ..
@@ -1307,120 +1001,9 @@ proof -
     .
 qed
 
-lemma (in bfs_invar) white_not_white_foldD:
-  assumes "white s v"
-  assumes "\<not> white (fold G src s) v"
-  shows
-    "v \<in> set (G.adjacency G (Q_head (queue s)))"
-    "P_lookup (parent (fold G src s)) v = Some (Q_head (queue s))"
-proof -
-  show "v \<in> set (G.adjacency G (Q_head (queue s)))"
-    using assms
-    by (fastforce simp add: discovered_def lookup_parent_fold_cong)
-  thus "P_lookup (parent (fold G src s)) v = Some (Q_head (queue s))"
-    using assms
-    by (auto simp add: lookup_parent_fold_cong)
-qed
-
-lemma (in bfs_invar_not_DONE) white_not_white_foldD_2:
-  assumes "white s v"
-  assumes "\<not> white (fold G src s) v"
-  shows "d (parent (fold G src s)) v = d (parent (fold G src s)) (Q_head (queue s)) + 1"
-  using parent_fold assms
-  by (fastforce intro: white_not_white_foldD(2) parent_imp_d)
-
-lemmas (in bfs_invar_not_DONE) white_not_white_foldD =
-  white_not_white_foldD
-  white_not_white_foldD_2
-
-subsubsection \<open>@{thm bfs_invar.parent_imp_edge}\<close>
-
-lemma (in bfs_invar_not_DONE) parent_imp_edge_fold:
-  assumes "P_lookup (parent (fold G src s)) v = Some u"
-  shows "(u, v) \<in> G.dE G"
-proof (cases "P_lookup (parent s) v = Some u")
-  case True
-  thus ?thesis
-    by (intro parent_imp_edge)
-next
-  case False
-  thus ?thesis
-    using assms head_queueI_2 G.mem_adjacency_iff_edge
-    by (fastforce simp add: lookup_parent_fold_cong)
-qed
-
-subsubsection \<open>@{thm bfs_invar.not_white_if_mem_queue}\<close>
-
-lemma (in bfs_invar_not_DONE) not_white_if_mem_queue_fold:
-  assumes "v \<in> set (Q_list (queue (fold G src s)))"
-  shows "\<not> white (fold G src s) v"
-proof (cases "v \<in> set (Q_list (queue s))")
-  case True
-  thus ?thesis
-    by (intro not_white_if_mem_queue not_whiteD(1))
-next
-  case False
-  hence "v \<notin> set (Q_list (Q_tail (queue s)))"
-    using invar_queue list_queue_non_empty
-    by (auto simp add: Q.list_tail intro: list.set_sel(2))
-  hence "v \<in> set (G.adjacency G (Q_head (queue s))) \<and> \<not> discovered src (parent s) v"
-    using assms
-    by (simp add: list_queue_fold_cong)
-  thus ?thesis
-    using assms
-    by (fastforce simp add: discovered_def lookup_parent_fold_cong)
-qed
-
-subsubsection \<open>@{thm bfs_invar.not_white_if_parent}\<close>
-
-lemma (in bfs_invar_not_DONE) not_white_if_parent_fold:
-  assumes "P_lookup (parent (fold G src s)) v = Some u"
-  shows "\<not> white (fold G src s) u"
-proof (cases "P_lookup (parent s) v = Some u")
-  case True
-  thus ?thesis
-    by (intro not_white_if_parent not_whiteD(1))
-next
-  case False
-  hence "u = Q_head (queue s)"
-    using assms
-    by (intro head_queueI_2)
-  thus ?thesis
-    using not_white_head_queue
-    by (intro not_whiteD(1)) simp
-qed
-
-subsubsection \<open>@{thm bfs_invar.black_imp_adjacency_not_white}\<close>
-
-lemma (in bfs_invar_not_DONE) black_imp_adjacency_not_white_fold:
-  assumes "black (fold G src s) u"
-  assumes "(u, v) \<in> G.dE G"
-  shows "\<not> white (fold G src s) v"
-proof (induct s u rule: vertex_color_induct)
-  case white
-  thus ?case
-    using assms(1) whiteD
-    by blast
-next
-  case gray
-  hence "u = Q_head (queue s)"
-    using assms(1)
-    by (intro head_queueI) simp+
-  thus ?case
-    using assms(2)
-    by (simp add: discovered_def lookup_parent_fold_cong override_on_def G.mem_adjacency_iff_edge)
-next
-  case black
-  thus ?case
-    using assms(2)
-    by (intro black_imp_adjacency_not_white not_whiteD(1))
-qed
-
-subsubsection \<open>@{thm bfs_invar.queue_sorted_wrt_d}\<close>
-
 lemma (in bfs_invar_not_DONE) queue_sorted_wrt_d_fold_aux:
   assumes u_mem_tail_queue: "u \<in> set (Q_list (Q_tail (queue s)))"
-  assumes v_mem_filter: "v \<in> set (filter (Not \<circ> discovered src (parent s)) (G.adjacency G (Q_head (queue s))))"
+  assumes v_mem_filter: "v \<in> set (filter (Not \<circ> is_discovered src (parent s)) (G.adjacency_list G (Q_head (queue s))))"
   shows "d (parent (fold G src s)) u \<le> d (parent (fold G src s)) v"
 proof -
   have u_mem_queue: "u \<in> set (Q_list (queue s))"
@@ -1428,13 +1011,13 @@ proof -
     by (auto simp add: Q.list_tail intro: list.set_sel(2))
   have "d (parent (fold G src s)) u = d (parent s) u"
     using u_mem_queue not_white_if_mem_queue
-    by (simp add: not_whiteD(3))
+    by (simp add: not_white_imp_rev_follow_fold_eq_rev_follow)
   also have "... \<le> d (parent s) (last (Q_list (queue s)))"
     using u_mem_queue
     by (intro mem_queue_imp_d_le)
   also have "... = d (parent (fold G src s)) (last (Q_list (queue s)))"
     using list_queue_non_empty not_white_if_mem_queue
-    by (simp add: not_whiteD(3))
+    by (simp add: not_white_imp_rev_follow_fold_eq_rev_follow)
   also have "... \<le> d (parent (fold G src s)) v"
     using v_mem_filter
     by (intro mem_filterD(2))
@@ -1448,26 +1031,26 @@ proof -
   let ?P = "\<lambda>u v. d (parent (fold G src s)) u \<le> d (parent (fold G src s)) v"
   have "sorted_wrt ?P (Q_list (queue s))"
     using queue_sorted_wrt_d not_white_if_mem_queue sorted_wrt_mono_rel[of "(Q_list (queue s))"]
-    by (simp add: not_whiteD(3))
+    by (simp add: not_white_imp_rev_follow_fold_eq_rev_follow)
   hence "sorted_wrt ?P (Q_list (Q_tail (queue s)))"
     by (simp add: Q.list_queue[OF invar_queue list_queue_non_empty])
-  moreover have "sorted_wrt ?P (filter (Not \<circ> discovered src (parent s)) (G.adjacency G (Q_head (queue s))))"
+  moreover have "sorted_wrt ?P (filter (Not \<circ> is_discovered src (parent s)) (G.adjacency_list G (Q_head (queue s))))"
     by (auto simp add: mem_filterD(1) intro: sorted_wrt_if)
   moreover have
     "\<forall>u\<in>set (Q_list (Q_tail (queue s))).
-      \<forall>v\<in>set (filter (Not \<circ> discovered src (parent s)) (G.adjacency G (Q_head (queue s)))).
+      \<forall>v\<in>set (filter (Not \<circ> is_discovered src (parent s)) (G.adjacency_list G (Q_head (queue s)))).
        d (parent (fold G src s)) u \<le> d (parent (fold G src s)) v"
     by (blast intro: queue_sorted_wrt_d_fold_aux)
   ultimately show ?thesis 
     by (simp add: list_queue_fold_cong sorted_wrt_append)
 qed
 
-subsubsection \<open>@{thm bfs_invar.d_last_queue_le}\<close>
+text \<open>Then the tenth invariant, @{thm bfs_invar.d_last_queue_le}.\<close>
 
 lemma (in bfs_invar_not_DONE) d_last_queue_le_fold_aux:
   assumes "\<not> Q_is_empty (queue (fold G src s))"
   shows "d (parent (fold G src s)) (last (Q_list (queue (fold G src s)))) \<le> d (parent (fold G src s)) (Q_head (queue s)) + 1"
-proof (cases "filter (Not \<circ> discovered src (parent s)) (G.adjacency G (Q_head (queue s))) = []")
+proof (cases "filter (Not \<circ> is_discovered src (parent s)) (G.adjacency_list G (Q_head (queue s))) = []")
   case True
   hence list_tail_non_empty: "Q_list (Q_tail (queue s)) \<noteq> []"
     using invar_G invar_queue not_DONE invar_queue_fold_2 assms
@@ -1481,24 +1064,44 @@ proof (cases "filter (Not \<circ> discovered src (parent s)) (G.adjacency G (Q_h
     by (simp add: Q.list_queue[OF invar_queue list_queue_non_empty])
   hence "d (parent (fold G src s)) (last (Q_list (queue (fold G src s)))) = d (parent s) (last (Q_list (queue s)))"
     using list_queue_non_empty not_white_if_mem_queue
-    by (simp add: not_whiteD(3))
+    by (simp add: not_white_imp_rev_follow_fold_eq_rev_follow)
   also have "... \<le> d (parent s) (Q_head (queue s)) + 1"
     using invar_queue list_queue_non_empty d_last_queue_le
     by (simp add: Q.is_empty)
   also have "... = d (parent (fold G src s)) (Q_head (queue s)) + 1"
     using not_white_head_queue
-    by (simp add: not_whiteD(3))
+    by (simp add: not_white_imp_rev_follow_fold_eq_rev_follow)
   finally show ?thesis
     .
 next
   case False
   hence
     "last (Q_list (queue (fold G src s))) \<in>
-     set (filter (Not \<circ> discovered src (parent s)) (G.adjacency G (Q_head (queue s))))"
+     set (filter (Not \<circ> is_discovered src (parent s)) (G.adjacency_list G (Q_head (queue s))))"
     unfolding list_queue_fold_cong last_appendR[OF False]
     by (intro last_in_set)
   thus ?thesis
     by (simp add: mem_filterD(1))
+qed
+
+lemma (in bfs_invar) mem_queue_imp_d_ge:
+  assumes "v \<in> set (Q_list (queue s))"
+  shows "d (parent s) (Q_head (queue s)) \<le> d (parent s) v"
+proof (cases "v = Q_head (queue s)")
+  case True
+  thus ?thesis
+    by simp
+next
+  case False
+  have "\<not> Q_is_empty (queue s)"
+    using invar_queue assms
+    by (auto simp add: Q.is_empty)
+  moreover hence "Q_head (queue s) = hd (Q_list (queue s))"
+    using invar_queue Q.list_head
+    by (simp add: Q.is_empty)
+  ultimately show ?thesis
+    using queue_sorted_wrt_d assms False sorted_wrt_imp_hd
+    by fastforce
 qed
 
 lemma (in bfs_invar_not_DONE) d_last_queue_le_fold_aux_2:
@@ -1511,25 +1114,25 @@ proof (cases "Q_list (Q_tail (queue s)) = []")
     by (simp add: Q.is_empty Q.list_head)
   hence
     "Q_head (queue (fold G src s)) =
-     hd (filter (Not \<circ> discovered src (parent s)) (G.adjacency G (Q_head (queue s))))"
+     hd (filter (Not \<circ> is_discovered src (parent s)) (G.adjacency_list G (Q_head (queue s))))"
     by (simp add: True list_queue_fold_cong)
-  moreover have "filter (Not \<circ> discovered src (parent s)) (G.adjacency G (Q_head (queue s))) \<noteq> []"
+  moreover have "filter (Not \<circ> is_discovered src (parent s)) (G.adjacency_list G (Q_head (queue s))) \<noteq> []"
     using invar_G invar_queue not_DONE invar_queue_fold_2 assms
     by (simp add: True Q.is_empty list_queue_fold_cong)
   ultimately have head_queue_fold_mem_filter:
     "Q_head (queue (fold G src s)) \<in>
-     set (filter (Not \<circ> discovered src (parent s)) (G.adjacency G (Q_head (queue s))))"
+     set (filter (Not \<circ> is_discovered src (parent s)) (G.adjacency_list G (Q_head (queue s))))"
     using list.set_sel(1)
     by metis
 
   have "d (parent (fold G src s)) (Q_head (queue s)) = d (parent s) (Q_head (queue s))"
     using not_white_head_queue
-    by (simp add: not_whiteD(3))
+    by (simp add: not_white_imp_rev_follow_fold_eq_rev_follow)
   also have "... \<le> d (parent s) (last (Q_list (queue s)))"
     by (intro head_queue_mem_queue mem_queue_imp_d_le)
   also have "... = d (parent (fold G src s)) (last (Q_list (queue s)))"
     using list_queue_non_empty not_white_if_mem_queue
-    by (simp add: not_whiteD(3))
+    by (simp add: not_white_imp_rev_follow_fold_eq_rev_follow)
   also have "... \<le> d (parent (fold G src s)) (Q_head (queue (fold G src s)))"
     using head_queue_fold_mem_filter
     by (intro mem_filterD(2))
@@ -1549,13 +1152,13 @@ next
 
   have "d (parent (fold G src s)) (Q_head (queue s)) = d (parent s) (Q_head (queue s))"
     using not_white_head_queue
-    by (simp add: not_whiteD(3))
+    by (simp add: not_white_imp_rev_follow_fold_eq_rev_follow)
   also have "... \<le> d (parent s) (Q_head (queue (fold G src s)))"
     using head_queue_fold_mem_queue
     by (intro mem_queue_imp_d_ge)
   also have "... = d (parent (fold G src s)) (Q_head (queue (fold G src s)))"
     using head_queue_fold_mem_queue not_white_if_mem_queue
-    by (simp add: not_whiteD(3))
+    by (simp add: not_white_imp_rev_follow_fold_eq_rev_follow)
   finally show ?thesis
     .
 qed
@@ -1574,7 +1177,7 @@ proof -
     .
 qed
 
-subsubsection \<open>@{thm bfs_invar.d_triangle_inequality}\<close>
+text \<open>Finally, the eleventh invariant, @{thm bfs_invar.d_triangle_inequality}.\<close>
 
 lemma (in bfs_invar) white_imp_gray_ancestor:
   assumes "dpath_bet (G.dE G) p u w"
@@ -1620,6 +1223,45 @@ next
   qed
 qed
 
+lemma (in bfs_invar) white_not_white_foldD:
+  assumes "white s v"
+  assumes "\<not> white (fold G src s) v"
+  shows
+    "v \<in> set (G.adjacency_list G (Q_head (queue s)))"
+    "P_lookup (parent (fold G src s)) v = Some (Q_head (queue s))"
+proof -
+  show "v \<in> set (G.adjacency_list G (Q_head (queue s)))"
+    using assms
+    by (fastforce simp add: is_discovered_def lookup_parent_fold_cong)
+  thus "P_lookup (parent (fold G src s)) v = Some (Q_head (queue s))"
+    using assms
+    by (auto simp add: lookup_parent_fold_cong)
+qed
+
+lemma (in bfs_valid_input) parent_imp_d:
+  assumes "Parent_Relation.parent (P_lookup (parent s))"
+  assumes "P_lookup (parent s) v = Some u"
+  shows "d (parent s) v = d (parent s) u + 1"
+proof -
+  have "rev_follow (parent s) v = rev_follow (parent s) u @ [v]"
+    using assms
+    by (simp add: parent.follow_psimps)
+  thus ?thesis
+    using parent.follow_non_empty[OF assms(1)]
+    by (simp add: dpath_length_snoc)
+qed
+
+lemma (in bfs_invar_not_DONE) white_not_white_foldD_2:
+  assumes "white s v"
+  assumes "\<not> white (fold G src s) v"
+  shows "d (parent (fold G src s)) v = d (parent (fold G src s)) (Q_head (queue s)) + 1"
+  using parent_fold assms
+  by (fastforce intro: white_not_white_foldD(2) parent_imp_d)
+
+lemmas (in bfs_invar_not_DONE) white_not_white_foldD =
+  white_not_white_foldD
+  white_not_white_foldD_2
+
 lemma (in bfs_invar_not_DONE) d_triangle_inequality_fold:
   assumes dpath_p: "dpath_bet (G.dE G) p u v"
   assumes not_white_fold_u: "\<not> white (fold G src s) u"
@@ -1651,7 +1293,7 @@ proof -
       by (auto simp add: G.mem_adjacency_iff_edge intro: dpath_bet_ConsI)
     have "d (parent (fold G src s)) v = d (parent s) v"
       using white_not_white
-      by (simp add: not_whiteD(3))
+      by (simp add: not_white_imp_rev_follow_fold_eq_rev_follow)
     also have "... \<le> d (parent s) (Q_head (queue s)) + dpath_length (Q_head (queue s) # p)"
       using not_white_head_queue white_not_white dpath_Cons
       by (auto intro: d_triangle_inequality)
@@ -1660,7 +1302,7 @@ proof -
       by (simp add: dpath_length_Cons)
     also have "... = d (parent (fold G src s)) (Q_head (queue s)) + 1 + dpath_length p"
       using not_white_head_queue
-      by (simp add: not_whiteD(3))
+      by (simp add: not_white_imp_rev_follow_fold_eq_rev_follow)
     also have "... = d (parent (fold G src s)) u + dpath_length p"
       using white_not_white not_white_fold_u
       by (simp add: white_not_white_foldD(3))
@@ -1673,13 +1315,13 @@ proof -
       by (intro white_not_white_foldD(3)) simp
     also have "... = d (parent s) (Q_head (queue s)) + 1"
       using not_white_head_queue
-      by (auto simp add: not_whiteD(3))
+      by (auto simp add: not_white_imp_rev_follow_fold_eq_rev_follow)
     also have "... \<le> d (parent s) u + 1"
       using gray_white
       by (intro mem_queue_imp_d_ge add_right_mono) simp
     also have "... = d (parent (fold G src s)) u + 1"
       using gray_white
-      by (simp add: not_whiteD(3))
+      by (simp add: not_white_imp_rev_follow_fold_eq_rev_follow)
     also have "... \<le> d (parent (fold G src s)) u + dpath_length p"
       using dpath_p gray_white
       by (fastforce intro: dpath_length_geq_1I add_left_mono)
@@ -1706,7 +1348,7 @@ proof -
       by (intro white_not_white_foldD(3)) simp
     also have "... = d (parent s) (Q_head (queue s)) + 1"
       using not_white_head_queue
-      by (auto simp add: not_whiteD(3))
+      by (auto simp add: not_white_imp_rev_follow_fold_eq_rev_follow)
     also have "... \<le> d (parent s) w + 1"
       using gray_w
       by (intro mem_queue_imp_d_ge add_right_mono) simp
@@ -1718,31 +1360,29 @@ proof -
       by (fastforce simp add: dpath_length_p)
     also have "... = d (parent (fold G src s)) u + dpath_length p"
       using black_white
-      by (simp add: not_whiteD(3))
+      by (simp add: not_white_imp_rev_follow_fold_eq_rev_follow)
     finally show ?thesis
       .
   next
     case not_white_not_white
     hence "d (parent (fold G src s)) v = d (parent s) v"
-      by (simp add: not_whiteD(3))
+      by (simp add: not_white_imp_rev_follow_fold_eq_rev_follow)
     also have "... \<le> d (parent s) u + dpath_length p"
       using dpath_p not_white_not_white
       by (intro d_triangle_inequality) simp+
     also have "... = d (parent (fold G src s)) u + dpath_length p"
       using not_white_not_white
-      by (simp add: not_whiteD(3))
+      by (simp add: not_white_imp_rev_follow_fold_eq_rev_follow)
     finally show ?thesis
       .
   qed
 qed
 
-subsubsection \<open>\<close>
-
 lemma (in bfs_invar_not_DONE) bfs_invar_fold:
   shows "bfs_invar'' (fold G src s)"
 proof (standard, goal_cases)
   case 1
-  show ?case using follow_invar'_parent_fold .
+  show ?case using follow_invar_parent_fold .
 next
   case 2
   show ?case using invar_queue_fold .
@@ -1775,6 +1415,562 @@ next
   thus ?case by (intro d_triangle_inequality_fold)
 qed
 
+(* qq *)
+(* Next: termination. Then: correctness. *)
+
+subsection \<open>@{term "Q_list \<circ> queue"}\<close>
+
+
+
+subsection \<open>@{term "Q_head \<circ> queue"}\<close>
+
+lemma (in bfs) head_queue_mem_dV:
+  assumes "Q_invar (queue s)"
+  assumes "set (Q_list (queue s)) \<subseteq> G.dV G"
+  assumes "\<not> DONE s"
+  shows "Q_head (queue s) \<in> G.dV G"
+  using assms list_queue_non_empty
+  by (auto simp add: Q.list_head)
+
+section \<open>Basic Lemmas\<close>
+
+subsection \<open>@{term discover}\<close>
+
+subsubsection \<open>@{term queue}\<close>
+
+
+
+subsubsection \<open>@{term parent}\<close>
+
+
+
+subsection \<open>@{term traverse_edge}\<close>
+
+subsubsection \<open>@{term queue}\<close>
+
+
+
+subsubsection \<open>@{term "Q_list \<circ> queue"}\<close>
+
+
+
+subsubsection \<open>@{term "P_lookup \<circ> parent"}\<close>
+
+
+
+subsubsection \<open>@{term "P_invar \<circ> parent"}\<close>
+
+
+
+subsubsection \<open>@{term T}\<close>
+
+
+
+subsection \<open>@{term fold}\<close>
+
+subsubsection \<open>@{term "Q_invar \<circ> queue"}\<close>
+
+
+
+subsubsection \<open>@{term "Q_list \<circ> queue"}\<close>
+
+
+
+
+subsubsection \<open>@{term "set \<circ> Q_list \<circ> queue"}\<close>
+
+lemma (in bfs) queue_fold_subset_dV:
+  assumes "G.invar G"
+  assumes "Q_invar (queue s)"
+  assumes "P_invar (parent s)"
+  assumes "set (Q_list (queue s)) \<subseteq> G.dV G"
+  assumes "\<not> DONE s"
+  shows "set (Q_list (queue (fold G src s))) \<subseteq> G.dV G"
+proof
+  fix v
+  assume assm: "v \<in> set (Q_list (queue (fold G src s)))"
+  show "v \<in> G.dV G"
+  proof (cases "v \<in> set (filter (Not \<circ> is_discovered src (parent s)) (G.adjacency_list G (Q_head (queue s))))")
+    case True
+    thus ?thesis
+      using G.adjacency_subset_dV
+      by auto
+  next
+    case False
+    hence "v \<in> set (Q_list (Q_tail (queue s)))"
+      using assms assm
+      by (auto simp add: list_queue_fold_cong_2)
+    hence "v \<in> set (Q_list (queue s))"
+      using assms(2, 5) list_queue_non_empty
+      by (auto simp add: Q.list_tail intro: list.set_sel(2))
+    thus ?thesis
+      using assms(4)
+      by blast
+  qed
+qed
+
+subsubsection \<open>@{term parent}\<close>
+
+
+
+subsubsection \<open>@{term "P_invar \<circ> parent"}\<close>
+
+
+
+lemma (in bfs) dom_parent_fold_subset_dV:
+  assumes "P_invar (parent s)"
+  assumes "distinct l"
+  assumes "P.dom (parent s) \<subseteq> G.dV G"
+  assumes "set l \<subseteq> G.dV G"
+  shows "P.dom (parent (List.fold (traverse_edge src u) l s)) \<subseteq> G.dV G"
+proof
+  fix v
+  assume assm: "v \<in> P.dom (parent (List.fold (traverse_edge src u) l s))"
+  show "v \<in> G.dV G"
+  proof (cases "v \<in> set (filter (Not \<circ> is_discovered src (parent s)) l)")
+    case True
+    thus ?thesis
+      using assms(4)
+      by auto
+  next
+    case False
+    have "P_lookup (parent (List.fold (traverse_edge src u) l s)) v \<noteq> None"
+      using assm
+      by (simp add: P.dom_def)
+    hence "P_lookup (parent s) v \<noteq> None"
+      using assms(1, 2) False
+      by (simp add: lookup_parent_fold_cong)
+    thus ?thesis
+      using assms(3)
+      by (auto simp add: P.dom_def)
+  qed
+qed
+
+lemma (in bfs) dom_parent_fold_subset_dV_2:
+  assumes "G.invar G"
+  assumes "P_invar (parent s)"
+  assumes "P.dom (parent s) \<subseteq> G.dV G"
+  shows "P.dom (parent (fold G src s)) \<subseteq> G.dV G"
+  using assms G.adjacency_subset_dV
+  by (intro G.distinct_adjacency_list dom_parent_fold_subset_dV) simp+
+
+lemma (in bfs) ran_parent_fold_cong:
+  assumes "G.invar G"
+  assumes "P_invar (parent s)"
+  shows
+    "P.ran (parent (fold G src s)) =
+     P.ran (parent s) \<union>
+     (if set (filter (Not \<circ> is_discovered src (parent s)) (G.adjacency_list G (Q_head (queue s)))) = {}
+      then {}
+      else {Q_head (queue s)})"
+proof
+  let ?S = "set (filter (Not \<circ> is_discovered src (parent s)) (G.adjacency_list G (Q_head (queue s))))"
+  show "P.ran (parent (fold G src s)) \<subseteq> P.ran (parent s) \<union> (if ?S = {} then {} else {Q_head (queue s)})"
+    using assms
+    by (auto simp add: P.ran_def lookup_parent_fold_cong_2 override_on_def)
+  show "P.ran (parent s) \<union> (if ?S = {} then {} else {Q_head (queue s)}) \<subseteq> P.ran (parent (fold G src s))"
+  proof
+    fix u
+    assume assm: "u \<in> P.ran (parent s) \<union> (if ?S = {} then {} else {Q_head (queue s)})"
+    show "u \<in> P.ran (parent (fold G src s))"
+    proof (cases "u \<in> P.ran (parent s)")
+      case True
+      then obtain v where
+        "P_lookup (parent s) v = Some u"
+        by (auto simp add: P.ran_def)
+      moreover hence "is_discovered src (parent s) v"
+        by (simp add: is_discovered_def)
+      ultimately show ?thesis
+        using assms
+        by (auto simp add: P.ran_def lookup_parent_fold_cong_2 override_on_def)
+    next
+      case False
+      then obtain v where
+        "v \<in> ?S"
+        using assm
+        by (auto split: if_splits(2))
+      moreover have "u = Q_head (queue s)"
+        using assm False
+        by (simp split: if_splits(2))
+      ultimately show ?thesis
+        using assms
+        by (auto simp add: P.ran_def lookup_parent_fold_cong_2 override_on_def)
+    qed
+  qed
+qed
+
+subsubsection \<open>@{term T}\<close>
+
+
+
+
+
+section \<open>Termination\<close>
+
+lemma (in bfs) loop_dom_aux:
+  assumes "G.invar G"
+  assumes "P_invar (parent s)"
+  assumes "P.dom (parent s) \<subseteq> G.dV G"
+  shows
+    "card (P.dom (parent (fold G src s))) =
+     card (P.dom (parent s)) +
+     card (set (filter (Not \<circ> is_discovered src (parent s)) (G.adjacency_list G (Q_head (queue s)))))"
+proof -
+  let ?S = "set (filter (Not \<circ> is_discovered src (parent s)) (G.adjacency_list G (Q_head (queue s))))"
+  have "P.dom (parent (fold G src s)) = P.dom (parent s) \<union> ?S"
+    using assms(1, 2)
+    by (auto simp add: P.dom_def lookup_parent_fold_cong_2 override_on_def)
+  moreover have "finite (P.dom (parent s))"
+    using assms(1, 3) finite_subset
+    by (fastforce intro: G.finite_dV)
+  moreover have "finite ?S"
+    by simp
+  moreover have "P.dom (parent s) \<inter> ?S = {}"
+    by (auto simp add: P.dom_def is_discovered_def)
+  ultimately show ?thesis
+    by (simp add: card_Un_disjoint)
+qed
+
+lemma (in bfs) loop_dom_aux_2:
+  assumes invar_G: "G.invar G"
+  assumes invar_queue: "Q_invar (queue s)"
+  assumes not_DONE: "\<not> DONE s"
+  assumes dom_parent_subset_dV: "P.dom (parent s) \<subseteq> G.dV G"
+  shows
+    "card (G.dV G) +
+     length (Q_list (Q_tail (queue s))) -
+     card (P.dom (parent s)) <
+     card (G.dV G) +
+     length (Q_list (queue s)) -
+     card (P.dom (parent s))"
+proof -
+  have "Q_list (queue s) \<noteq> []"
+    using invar_queue not_DONE
+    by (intro list_queue_non_empty)
+  hence "length (Q_list (Q_tail (queue s))) < length (Q_list (queue s))"
+    using invar_queue
+    by (simp add: Q.list_tail)
+  moreover have "card (P.dom (parent s)) \<le> card (G.dV G)"
+    using invar_G dom_parent_subset_dV
+    by (intro G.finite_dV card_mono)
+  ultimately show ?thesis
+    by simp
+qed
+
+lemma (in bfs) loop_dom:
+  assumes "G.invar G"
+  assumes "Q_invar (queue s)"
+  assumes "P_invar (parent s)"
+  assumes "set (Q_list (queue s)) \<subseteq> G.dV G"
+  assumes "P.dom (parent s) \<subseteq> G.dV G"
+  shows "loop_dom (G, src, s)"
+  using assms
+proof (induct "card (G.dV G) + length (Q_list (queue s)) - card (P.dom (parent s))"
+       arbitrary: s
+       rule: less_induct)
+  case less
+  show ?case
+  proof (cases "DONE s")
+    case True
+    thus ?thesis
+      by (blast intro: loop.domintros)
+  next
+    case False
+    let ?u = "Q_head (queue s)"
+    let ?q = "Q_tail (queue s)"
+    let ?S = "set (filter (Not \<circ> is_discovered src (parent s)) (G.adjacency_list G (Q_head (queue s))))"
+
+    have "length (Q_list (queue (fold G src s))) = length (Q_list ?q) + card ?S"
+      using less.prems(1-3) False G.distinct_adjacency_list
+      by (simp add: list_queue_fold_cong_2 distinct_card[symmetric])
+    moreover have "card (P.dom (parent (fold G src s))) = card (P.dom (parent s)) + card ?S"
+      using less.prems(1, 3, 5)
+      by (intro loop_dom_aux)
+    ultimately have
+      "card (G.dV G) + length (Q_list (queue (fold G src s))) - card (P.dom (parent (fold G src s))) =
+       card (G.dV G) + length (Q_list ?q) + card ?S - (card (P.dom (parent s)) + card ?S)"
+      by presburger
+    also have "... = card (G.dV G) + length (Q_list ?q) - card (P.dom (parent s))"
+      by simp
+    also have "... < card (G.dV G) + length (Q_list (queue s)) - card (P.dom (parent s))"
+      using less.prems False
+      by (intro loop_dom_aux_2)
+    finally have
+      "card (G.dV G) + length (Q_list (queue (fold G src s))) - card (P.dom (parent (fold G src s))) <
+       card (G.dV G) + length (Q_list (queue s)) - card (P.dom (parent s))"
+      .
+    thus ?thesis
+      using less.prems
+      by (intro invar_queue_fold_2 invar_parent_fold_2 queue_fold_subset_dV dom_parent_fold_subset_dV_2 less.hyps loop.domintros)
+  qed
+qed
+
+section \<open>Invariants\<close>
+
+subsection \<open>Definitions\<close>
+
+(* TODO Rename. *)
+
+
+
+locale bfs_invar_DONE = bfs_invar where P_update = P_update and Q_snoc = Q_snoc for
+  P_update :: "'a::linorder \<Rightarrow> 'a \<Rightarrow> 'm \<Rightarrow> 'm" and
+  Q_snoc :: "'q \<Rightarrow> 'a \<Rightarrow> 'q" +
+  assumes DONE: "DONE s"
+
+
+
+
+
+
+
+abbreviation (in bfs) bfs_invar_DONE' :: "'n \<Rightarrow> 'a \<Rightarrow> ('q, 'm) state \<Rightarrow> bool" where
+  "bfs_invar_DONE' G src s \<equiv>
+   bfs_invar_DONE
+    Map_empty Map_delete Map_lookup Map_inorder Map_inv
+    Set_empty Set_insert Set_delete Set_isin Set_inorder Set_inv
+    P_empty P_delete P_lookup P_invar
+    Q_empty Q_is_empty Q_head Q_tail Q_invar Q_list
+    Map_update G src s P_update Q_snoc"
+
+abbreviation (in bfs_valid_input) bfs_invar_DONE'' :: "('q, 'm) state \<Rightarrow> bool" where
+  "bfs_invar_DONE'' \<equiv> bfs_invar_DONE' G src"
+
+subsection \<open>Convenience Lemmas\<close>
+
+subsubsection \<open>@{term bfs}\<close>
+
+lemma (in bfs) bfs_invar_not_DONE'I:
+  assumes "bfs_invar' G src s"
+  assumes "\<not> DONE s"
+  shows "bfs_invar_not_DONE' G src s"
+  using assms
+  by (simp add: bfs_invar_not_DONE_def bfs_invar_not_DONE_axioms_def)
+
+lemma (in bfs) bfs_invar_DONE'I:
+  assumes "bfs_invar' G src s"
+  assumes "DONE s"
+  shows "bfs_invar_DONE' G src s"
+  using assms
+  by (simp add: bfs_invar_DONE_def bfs_invar_DONE_axioms_def)
+
+lemma (in bfs) rev_follow_non_empty:
+  assumes "Parent_Relation.parent (P_lookup m)"
+  shows "rev_follow m v \<noteq> []"
+  using assms
+  by (auto dest: parent.follow_non_empty)
+
+lemma (in bfs) distinct_rev_follow:
+  assumes "Parent_Relation.parent (P_lookup m)"
+  shows "distinct (rev_follow m v)"
+  unfolding distinct_rev
+  using assms
+  by (intro parent.distinct_follow)
+
+lemma (in bfs) last_rev_follow:
+  assumes "Parent_Relation.parent (P_lookup m)"
+  shows "last (rev_follow m v) = v"
+proof -
+  let ?l = "parent.follow (P_lookup m) v"
+  have "?l = hd ?l # tl ?l"
+    using assms
+    by (intro parent.follow_non_empty hd_Cons_tl[symmetric])
+  hence "hd ?l = v"
+    using assms
+    by (auto dest: parent.follow_ConsD)
+  thus ?thesis
+    using assms parent.follow_non_empty
+    by (fastforce simp add: last_rev)
+qed
+
+subsubsection \<open>@{term bfs_valid_input}\<close>
+
+context bfs_valid_input
+begin
+sublocale finite_dgraph "G.dE G"
+proof (standard, goal_cases)
+  case 1
+  show ?case
+    using invar_G
+    by (intro G.finite_dE)
+qed
+end
+
+
+
+
+
+subsubsection \<open>@{term bfs_invar}\<close>
+
+lemma (in bfs_invar) distinct_rev_follow:
+  shows "distinct (rev_follow (parent s) v)"
+  using distinct_follow
+  by simp
+
+subsection \<open>Basic Lemmas\<close>
+
+subsubsection \<open>@{term bfs_valid_input}\<close>
+
+
+
+subsubsection \<open>@{term bfs_invar}\<close>
+
+lemma (in bfs_invar) not_white_imp_dpath_rev_follow:
+  assumes "\<not> white s v"
+  shows "dpath_bet (G.dE G) (rev_follow (parent s) v) src v"
+  using assms
+proof (induct v rule: follow_pinduct)
+  case (1 v)
+  show ?case
+  proof (cases "v = src")
+    case True
+    thus ?thesis
+      using parent_src src_mem_dV
+      by (auto simp add: G.dE_def G.dV_def follow_psimps intro: dpath_bet_reflexive)
+  next
+    case False
+    then obtain u where
+      u: "P_lookup (parent s) v = Some u"
+      using "1.prems"
+      by (auto simp add: is_discovered_def)
+    hence
+      "follow v = v # follow u"
+      "(u, v) \<in> G.dE G"
+      "\<not> white s u"
+      using not_white_if_parent
+      by (auto simp add: follow_psimps intro: parent_imp_edge)
+    moreover hence "dpath_bet (G.dE G) (rev_follow (parent s) u) src u"
+      using u
+      by (intro "1.hyps")
+    ultimately show ?thesis
+      by (auto intro: dpath_bet_snocI)
+  qed
+qed
+
+lemma (in bfs_invar) hd_rev_follow_eq_src:
+  assumes "\<not> white s v"
+  shows "hd (rev_follow (parent s) v) = src"
+  using assms
+  by (intro hd_of_dpath_bet'[symmetric]) (rule not_white_imp_dpath_rev_follow)
+
+
+
+
+
+lemma (in bfs_invar) d_triangle_inequality_edge:
+  assumes "(u, v) \<in> G.dE G"
+  assumes "\<not> white s u"
+  assumes "\<not> white s v"
+  shows "d (parent s) v \<le> d (parent s) u + 1"
+proof -
+  have "dpath_bet (G.dE G) [u, v] u v"
+    using assms(1)
+    by (intro edges_are_dpath_bet)
+  thus ?thesis
+    using assms(2, 3)
+    using d_triangle_inequality
+    by fastforce
+qed
+
+subsection \<open>@{term bfs.init}\<close>
+
+subsubsection \<open>\<close>
+
+
+
+subsubsection \<open>\<close>
+
+
+
+subsection \<open>@{term bfs.fold}\<close>
+
+subsubsection \<open>Convenience Lemmas\<close>
+
+
+
+
+
+
+
+
+
+
+
+
+
+subsubsection \<open>\<close>
+
+
+
+
+
+subsubsection \<open>@{thm bfs_invar.invar_queue}\<close>
+
+
+
+subsubsection \<open>@{thm bfs_invar.invar_parent}\<close>
+
+
+
+subsubsection \<open>@{thm bfs_invar.parent_src}\<close>
+
+
+
+subsubsection \<open>Basic Lemmas\<close>
+
+
+
+
+
+
+
+
+
+
+
+
+
+lemmas (in bfs_invar_not_DONE) not_whiteD =
+  not_white_imp_not_white_fold
+  not_white_imp_lookup_parent_fold_eq_lookup_parent
+  not_white_imp_rev_follow_fold_eq_rev_follow
+
+
+
+
+
+subsubsection \<open>@{thm bfs_invar.parent_imp_edge}\<close>
+
+
+
+subsubsection \<open>@{thm bfs_invar.not_white_if_mem_queue}\<close>
+
+
+
+subsubsection \<open>@{thm bfs_invar.not_white_if_parent}\<close>
+
+
+
+subsubsection \<open>@{thm bfs_invar.black_imp_adjacency_not_white}\<close>
+
+
+
+subsubsection \<open>@{thm bfs_invar.queue_sorted_wrt_d}\<close>
+
+
+
+subsubsection \<open>@{thm bfs_invar.d_last_queue_le}\<close>
+
+
+
+subsubsection \<open>@{thm bfs_invar.d_triangle_inequality}\<close>
+
+
+
+subsubsection \<open>\<close>
+
+
+
 section \<open>Correctness\<close>
 
 subsection \<open>Definitions\<close>
@@ -1782,15 +1978,15 @@ subsection \<open>Definitions\<close>
 abbreviation (in bfs) dist :: "'n \<Rightarrow> 'a \<Rightarrow> 'a \<Rightarrow> enat" where
   "dist G \<equiv> Shortest_Dpath.dist (G.dE G)"
 
-abbreviation (in bfs) shortest_dpath :: "'n \<Rightarrow> 'a list \<Rightarrow> 'a \<Rightarrow> 'a \<Rightarrow> bool" where
-  "shortest_dpath G p u v \<equiv> dpath_bet (G.dE G) p u v \<and> dpath_length p = dist G u v"
+abbreviation (in bfs) is_shortest_dpath :: "'n \<Rightarrow> 'a list \<Rightarrow> 'a \<Rightarrow> 'a \<Rightarrow> bool" where
+  "is_shortest_dpath G p u v \<equiv> dpath_bet (G.dE G) p u v \<and> dpath_length p = dist G u v"
 
 subsection \<open>Basic Lemmas\<close>
 
 lemma (in bfs_invar) queue_subset_dV:
   shows "set (Q_list (queue s)) \<subseteq> G.dV G"
   using not_white_if_mem_queue not_white_imp_dpath_rev_follow
-  by (auto intro: dpath_bet_endpoints(2))
+  by (auto simp add: G.dV_def intro: dpath_bet_endpoints(2))
 
 lemma (in bfs_invar) dom_parent_subset_dV:
   shows "P.dom (parent s) \<subseteq> G.dV G"
@@ -1886,9 +2082,9 @@ proof
   qed
 qed
 
-lemma (in bfs_invar_tbd) completeness:
+lemma (in bfs_valid_input) completeness:
   assumes "bfs_invar'' s"
-  assumes "\<not> discovered src (parent (loop G src s)) v"
+  assumes "\<not> is_discovered src (parent (loop G src s)) v"
   shows "\<not> reachable (G.dE G) src v"
   using assms
 proof (induct rule: bfs_induct[OF assms(1)])
@@ -1923,8 +2119,8 @@ proof -
     using assms
     by (auto simp add: reachable_iff_dpath_bet intro: not_white_imp_dpath_rev_follow)
   then obtain p where
-    "shortest_dpath G p src v"
-    by (elim shortest_dpath_if_reachable_2) simp+
+    "is_shortest_dpath G p src v"
+    by (elim is_shortest_dpath_if_reachable_2) simp+
   thus ?thesis
     using assms
   proof (induct p arbitrary: v rule: dpath_rev_induct)
@@ -1945,15 +2141,15 @@ proof -
         by (metis white_imp_not_reachable dist_eq_\<delta> \<delta>_reachable_conv)
       thus ?thesis
         using "3.prems"(1)
-        by (auto intro: shortest_dpathE_2)
+        by (auto intro: is_shortest_dpathE_2)
     next
       case False
-      have shortest_dpath: "shortest_dpath G (l @ [u]) src u"
+      have is_shortest_dpath: "is_shortest_dpath G (l @ [u]) src u"
         using "3.prems"(1)
         by
           (auto
-           simp add: dpath_length_eq_dpath_weight dist_eq_\<delta> shortest_dpath_def[symmetric]
-           intro: shortest_dpath_prefI)
+           simp add: dpath_length_eq_dpath_weight dist_eq_\<delta> is_shortest_dpath_def[symmetric]
+           intro: is_shortest_dpath_prefI)
       have "(u, v) \<in> G.dE G"
         using "3.prems"(1) last_of_dpath_bet
         by (fastforce simp add: edge_iff_dpath_bet intro: split_dpath)
@@ -1961,21 +2157,21 @@ proof -
         using False "3.prems"(2)
         by (intro d_triangle_inequality_edge)
       also have "... \<le> dist G src u + 1"
-        using "3.hyps"[OF shortest_dpath False]
+        using "3.hyps"[OF is_shortest_dpath False]
         unfolding plus_enat_simps(1)[symmetric] one_enat_def[symmetric]
         by (intro add_right_mono)
       also have "... = dist G src v"
         using "3.prems"(1)
-        by (auto intro: shortest_dpathE_2)
+        by (auto intro: is_shortest_dpathE_2)
       finally show ?thesis
         by simp
     qed
   qed
 qed
 
-lemma (in bfs_invar_DONE) not_white_imp_shortest_dpath:
+lemma (in bfs_invar_DONE) not_white_imp_is_shortest_dpath:
   assumes "\<not> white s v"
-  shows "shortest_dpath G (rev_follow (parent s) v) src v"
+  shows "is_shortest_dpath G (rev_follow (parent s) v) src v"
 proof (rule conjI)
   show "dpath_bet (G.dE G) (rev_follow (parent s) v) src v"
     using assms
@@ -1985,10 +2181,10 @@ proof (rule conjI)
     by (intro not_white_imp_d_le_dist dist_le_dpath_length antisym)
 qed
 
-lemma (in bfs_invar_tbd) soundness:
+lemma (in bfs_valid_input) soundness:
   assumes "bfs_invar'' s"
-  assumes "discovered src (parent (loop G src s)) v"
-  shows "shortest_dpath G (rev_follow (parent (loop G src s)) v) src v"
+  assumes "is_discovered src (parent (loop G src s)) v"
+  shows "is_shortest_dpath G (rev_follow (parent (loop G src s)) v) src v"
   using assms
 proof (induct rule: bfs_induct[OF assms(1)])
   case (1 G src s)
@@ -2000,7 +2196,7 @@ proof (induct rule: bfs_induct[OF assms(1)])
       by (intro bfs_invar_DONE'I)
     thus ?thesis
       using "1.prems"(2)
-      by (intro bfs_invar_DONE.not_white_imp_shortest_dpath) (simp_all add: bfs_invar_DONE.loop_psimps)
+      by (intro bfs_invar_DONE.not_white_imp_is_shortest_dpath) (simp_all add: bfs_invar_DONE.loop_psimps)
   next
     case False
     with "1.prems"(1)
@@ -2014,26 +2210,26 @@ qed
 
 subsection \<open>Correctness\<close>
 
-abbreviation (in bfs) shortest_dpath_Map :: "'n \<Rightarrow> 'a \<Rightarrow> 'm \<Rightarrow> bool" where
-  "shortest_dpath_Map G src m \<equiv>
-   \<forall>v. (discovered src m v \<longrightarrow> shortest_dpath G (rev_follow m v) src v) \<and>
-       (\<not> discovered src m v \<longrightarrow> \<not> reachable (G.dE G) src v)"
+abbreviation (in bfs) is_shortest_dpath_Map :: "'n \<Rightarrow> 'a \<Rightarrow> 'm \<Rightarrow> bool" where
+  "is_shortest_dpath_Map G src m \<equiv>
+   \<forall>v. (is_discovered src m v \<longrightarrow> is_shortest_dpath G (rev_follow m v) src v) \<and>
+       (\<not> is_discovered src m v \<longrightarrow> \<not> reachable (G.dE G) src v)"
 
-lemma (in bfs_invar_tbd) correctness:
+lemma (in bfs_valid_input) correctness:
   assumes "bfs_invar'' s"
-  shows "shortest_dpath_Map G src (parent (loop G src s))"
+  shows "is_shortest_dpath_Map G src (parent (loop G src s))"
   using assms soundness completeness
   by simp
 
-theorem (in bfs_invar_tbd) bfs_correct:
-  shows "shortest_dpath_Map G src (bfs G src)"
+theorem (in bfs_valid_input) bfs_correct:
+  shows "is_shortest_dpath_Map G src (bfs G src)"
   using bfs_invar_init
   by (intro correctness)
 
 corollary (in bfs) bfs_correct:
-  assumes "bfs_invar_tbd' G src"
-  shows "shortest_dpath_Map G src (bfs G src)"
+  assumes "bfs_valid_input' G src"
+  shows "is_shortest_dpath_Map G src (bfs G src)"
   using assms
-  by (intro bfs_invar_tbd.bfs_correct)
+  by (intro bfs_valid_input.bfs_correct)
 
 end
