BFS/Undirected_BFS.thy
@@ -1,13 +1,13 @@
 theory Undirected_BFS
   imports
-    "../Graph_Theory/Adaptors/Adjacency_Adaptor"
+    "../Graph/Adjacency/Adjacency_Adaptor"
     BFS
-    "../Graph_Theory/Adaptors/Shortest_Path_Adaptor"
+    "../Graph/Adaptors/Shortest_Path_Adaptor"
 begin
 
 section \<open>Invariants\<close>
 
-locale undirected_bfs_invar_tbd = bfs where
+locale undirected_bfs_valid_input = bfs where
   Map_update = Map_update and
   P_update = P_update and
   Q_snoc = Q_snoc for
@@ -17,7 +17,7 @@ locale undirected_bfs_invar_tbd = bfs where
   fixes G :: 'n
   fixes src :: 'a
   assumes invar_G: "G.invar G"
-  assumes symmetric: "v \<in> set (G.adjacency G u) \<longleftrightarrow> u \<in> set (G.adjacency G v)"
+  assumes symmetric: "v \<in> set (G.adjacency_list G u) \<longleftrightarrow> u \<in> set (G.adjacency_list G v)"
   assumes src_mem_V: "src \<in> G.V G"
 begin
 
@@ -30,7 +30,7 @@ next
   show ?case using symmetric .
 qed
 
-sublocale bfs_invar_tbd
+sublocale bfs_valid_input
 proof (standard, goal_cases)
   case 1
   show ?case
@@ -45,9 +45,9 @@ qed
 
 end
 
-abbreviation (in bfs) undirected_bfs_invar_tbd' :: "'n \<Rightarrow> 'a \<Rightarrow> bool" where
-  "undirected_bfs_invar_tbd' G src \<equiv>
-   undirected_bfs_invar_tbd
+abbreviation (in bfs) undirected_bfs_valid_input' :: "'n \<Rightarrow> 'a \<Rightarrow> bool" where
+  "undirected_bfs_valid_input' G src \<equiv>
+   undirected_bfs_valid_input
     Map_empty Map_delete Map_lookup Map_inorder Map_inv
     Set_empty Set_insert Set_delete Set_isin Set_inorder Set_inv
     P_empty P_delete P_lookup P_invar
@@ -56,39 +56,39 @@ abbreviation (in bfs) undirected_bfs_invar_tbd' :: "'n \<Rightarrow> 'a \<Righta
 
 section \<open>Correctness\<close>
 
-abbreviation (in bfs) shortest_path_Map :: "'n \<Rightarrow> 'a \<Rightarrow> 'm \<Rightarrow> bool" where
-  "shortest_path_Map G src m \<equiv>
-   \<forall>v. (discovered src m v \<longrightarrow> shortest_path (G.E G) (rev_follow m v) src v) \<and>
-       (\<not> discovered src m v \<longrightarrow> \<not> reachable (G.E G) src v)"
+abbreviation (in bfs) is_shortest_path_Map :: "'n \<Rightarrow> 'a \<Rightarrow> 'm \<Rightarrow> bool" where
+  "is_shortest_path_Map G src m \<equiv>
+   \<forall>v. (is_discovered src m v \<longrightarrow> is_shortest_path (G.E G) (rev_follow m v) src v) \<and>
+       (\<not> is_discovered src m v \<longrightarrow> \<not> reachable (G.E G) src v)"
 
-lemma (in undirected_bfs_invar_tbd) dist_eq_dist:
+lemma (in undirected_bfs_valid_input) dist_eq_dist:
   shows "Shortest_Path.dist (G.E G) u v = dist G u v"
   using dist_eq_dist
   by (simp add: dE_eq_dEs)
 
-lemma (in undirected_bfs_invar_tbd) shortest_path_iff_shortest_dpath:
-  shows "shortest_path (G.E G) p u v \<longleftrightarrow> shortest_dpath G p u v"
+lemma (in undirected_bfs_valid_input) is_shortest_path_iff_is_shortest_dpath:
+  shows "is_shortest_path (G.E G) p u v \<longleftrightarrow> is_shortest_dpath G p u v"
   by (simp add: walk_betw_iff_dpath_bet dE_eq_dEs path_length_eq_dpath_length dist_eq_dist)
 
-lemma (in undirected_bfs_invar_tbd) reachable_iff_reachable:
+lemma (in undirected_bfs_valid_input) reachable_iff_reachable:
   shows "reachable (G.E G) u v \<longleftrightarrow> Noschinski_to_DDFS.reachable (G.dE G) u v"
   using reachable_iff_reachable
   by (simp add: dE_eq_dEs)
 
-lemma (in undirected_bfs_invar_tbd) undirected_bfs_correct:
-  shows "shortest_path_Map G src (bfs G src)"
+lemma (in undirected_bfs_valid_input) undirected_bfs_correct:
+  shows "is_shortest_path_Map G src (bfs G src)"
 proof -
-  have "shortest_dpath_Map G src (bfs G src)"
+  have "is_shortest_dpath_Map G src (bfs G src)"
     using bfs_correct
     .
   thus ?thesis
-    by (simp add: shortest_path_iff_shortest_dpath reachable_iff_reachable)
+    by (simp add: is_shortest_path_iff_is_shortest_dpath reachable_iff_reachable)
 qed
 
 lemma (in bfs) undirected_bfs_correct:
-  assumes "undirected_bfs_invar_tbd' G src"
-  shows "shortest_path_Map G src (bfs G src)"
+  assumes "undirected_bfs_valid_input' G src"
+  shows "is_shortest_path_Map G src (bfs G src)"
   using assms
-  by (intro undirected_bfs_invar_tbd.undirected_bfs_correct)
+  by (intro undirected_bfs_valid_input.undirected_bfs_correct)
 
 end
