Graph_Theory/Directed_Graphs/Directed_Graphs.thy
@@ -1,7 +1,0 @@
-theory Directed_Graphs
-  imports
-    Directed_Adjacency
-    Shortest_Dpath
-begin
-
-end
